theories/zoo_saturn/inf_ws_queue_1.v
@@ -1,27 +1,26 @@
-From Coq.Logic Require Import
-  FunctionalExtensionality.
-
 From zoo Require Import
   prelude.
 From zoo.common Require Import
   countable
-  list.
+  function
+  relations.
 From zoo.iris.base_logic Require Import
   lib.excl
   lib.twins
+  lib.auth_twins
   lib.auth_nat_max
   lib.mono_list.
 From zoo.language Require Import
   notations.
 From zoo.program_logic Require Import
-  wise_prophet
-  identifier.
+  identifier
+  wise_prophets.
 From zoo.diaframe Require Import
   diaframe.
 From zoo_std Require Import
-  option
+  domain
   inf_array
-  domain.
+  option.
 From zoo_saturn Require Export
   base
   inf_ws_queue_1__code.
@@ -30,54 +29,70 @@ From zoo_saturn Require Import
 From zoo Require Import
   options.
 
-Implicit Types front : nat.
-Implicit Types back : Z.
-Implicit Types l slot : location.
-Implicit Types id : identifier.
+Implicit Types front back : nat.
+Implicit Types l : location.
+Implicit Types id : prophet_id.
 Implicit Types v t : val.
-Implicit Types vs hist : list val.
+Implicit Types vs ws hist lhist : list val.
 Implicit Types priv : nat → val.
+
+Inductive state :=
+  | Empty
+  | Nonempty
+  | Emptyish
+  | Superempty.
+Implicit Types state : state.
+
+#[local] Instance state_inhabited : Inhabited state :=
+  populate Empty.
+
+Inductive stability :=
+  | Stable
+  | Unstable.
+Implicit Types stable : stability.
+
+#[local] Instance stability_inhabited : Inhabited stability :=
+  populate Stable.
 
 #[local] Program Definition prophet := {|
   typed_prophet_type :=
-    nat * identifier ;
+    identifier ;
   typed_prophet_of_val v :=
     match v with
-    | ValTuple [ValInt front; ValId id] =>
-        Some (₊front, id)
+    | ValId id =>
+        Some id
     | _ =>
         None
     end ;
-  typed_prophet_to_val '(front, id) :=
-    (#front, #id)%V ;
+  typed_prophet_to_val id :=
+    #id ;
 |}.
 Solve Obligations of prophet with
   try done.
 Next Obligation.
-  intros (front & id) v ->. simplify. rewrite Nat2Z.id //.
+  naive_solver.
 Qed.
 Implicit Types past prophs : list prophet.(typed_prophet_type).
+Implicit Types pasts prophss : nat → list prophet.(typed_prophet_type).
 
 Class InfWsQueue1G Σ `{zoo_G : !ZooG Σ} := {
   #[local] inf_ws_queue_1_G_inf_array_G :: InfArrayG Σ ;
-  #[local] inf_ws_queue_1_G_ctl_G :: TwinsG Σ (ZO * (nat -d> val_O)) ;
+  #[local] inf_ws_queue_1_G_prophets_G :: WiseProphetsG Σ prophet ;
+  #[local] inf_ws_queue_1_G_model_G :: AuthTwinsG Σ (leibnizO (list val)) suffix ;
+  #[local] inf_ws_queue_1_G_owner_G :: TwinsG Σ (leibnizO (stability * nat * (nat → val))) ;
   #[local] inf_ws_queue_1_G_front_G :: AuthNatMaxG Σ ;
-  #[local] inf_ws_queue_1_G_hist_G :: MonoListG Σ val ;
-  #[local] inf_ws_queue_1_G_model_G :: TwinsG Σ (leibnizO (list val)) ;
-  #[local] inf_ws_queue_1_G_lock_G :: ExclG Σ unitO ;
-  #[local] inf_ws_queue_1_G_prophet_G :: WiseProphetG Σ prophet ;
-  #[local] inf_ws_queue_1_G_winner_G :: TwinsG Σ (natO * (val_O -d> ▶ ∙)) ;
+  #[local] inf_ws_queue_1_G_history_G :: MonoListG Σ val ;
+  #[local] inf_ws_queue_1_G_winner_G :: TwinsG Σ (natO * ▶ ∙) ;
 }.
 
 Definition inf_ws_queue_1_Σ := #[
   inf_array_Σ ;
-  twins_Σ (ZO * (nat -d> val_O)) ;
+  wise_prophets_Σ prophet ;
+  auth_twins_Σ (leibnizO (list val)) suffix ;
+  twins_Σ (leibnizO (stability * nat * (nat → val))) ;
   auth_nat_max_Σ ;
   mono_list_Σ val ;
-  twins_Σ (leibnizO (list val)) ;
-  excl_Σ unitO ;
-  wise_prophet_Σ prophet ;
-  twins_Σ (natO * (val_O -d> ▶ ∙))
+  twins_Σ (natO * ▶ ∙)
 ].
 #[global] Instance subG_inf_ws_queue_1_Σ Σ `{zoo_G : !ZooG Σ} :
   subG inf_ws_queue_1_Σ Σ →
@@ -89,230 +104,336 @@ Qed.
 Section inf_ws_queue_1_G.
   Context `{inf_ws_queue_1_G : InfWsQueue1G Σ}.
 
-  Implicit Types Φ : val → iProp Σ.
+  Implicit Types P : iProp Σ.
 
   Record metadata := {
     metadata_data : val ;
+    metadata_inv : namespace ;
     metadata_prophet : prophet_id ;
-    metadata_prophet_name : wise_prophet_name ;
-    metadata_ctl : gname ;
+    metadata_prophet_name : wise_prophets_name ;
+    metadata_model : auth_twins_name ;
+    metadata_owner : gname ;
     metadata_front : gname ;
-    metadata_hist : gname ;
-    metadata_model : gname ;
-    metadata_lock : gname ;
+    metadata_history : gname ;
     metadata_winner : gname ;
   }.
-  Implicit Types γ : metadata.
 
-  #[local] Instance metadata_eq_dec :
-    EqDecision metadata.
-  Proof.
-    solve_decision.
-  Qed.
+  #[local] Instance metadata_eq_dec : EqDecision metadata :=
+    ltac:(solve_decision).
   #[local] Instance metadata_countable :
     Countable metadata.
   Proof.
     solve_countable.
   Qed.
 
-  #[local] Definition clt₁' γ_ctl back priv :=
-    twins_twin1 (twins_G := inf_ws_queue_1_G_ctl_G) γ_ctl (DfracOwn 1) (back, priv).
-  #[local] Definition clt₁ γ back priv :=
-    clt₁' γ.(metadata_ctl) back priv.
-  #[local] Definition clt₂' γ_ctl back priv :=
-    twins_twin2 (twins_G := inf_ws_queue_1_G_ctl_G) γ_ctl (back, priv).
-  #[local] Definition clt₂ γ back priv :=
-    clt₂' γ.(metadata_ctl) back priv.
-
-  #[local] Definition front_auth' γ_front front :=
-    auth_nat_max_auth γ_front (DfracOwn 1) front.
-  #[local] Definition front_auth γ front :=
-    front_auth' γ.(metadata_front) front.
-  #[local] Definition front_lb γ front :=
-    auth_nat_max_lb γ.(metadata_front) front.
-
-  #[local] Definition history_auth' γ_history hist :=
-    mono_list_auth γ_history (DfracOwn 1) hist.
-  #[local] Definition history_auth γ hist :=
-    history_auth' γ.(metadata_hist) hist.
-  #[local] Definition history_at γ i v :=
-    mono_list_at γ.(metadata_hist) i v.
-
   #[local] Definition model₁' γ_model vs :=
-    twins_twin2 (twins_G := inf_ws_queue_1_G_model_G) γ_model vs.
-  #[local] Definition model₁ γ vs :=
-    model₁' γ.(metadata_model) vs.
+    auth_twins_twin1 _ γ_model vs.
+  #[local] Definition model₁ γ :=
+    model₁' γ.(metadata_model).
   #[local] Definition model₂' γ_model vs :=
-    twins_twin1 (twins_G := inf_ws_queue_1_G_model_G) γ_model (DfracOwn 1) vs.
-  #[local] Definition model₂ γ vs :=
-    model₂' γ.(metadata_model) vs.
+    auth_twins_twin2 _ γ_model vs.
+  #[local] Definition model₂ γ :=
+    model₂' γ.(metadata_model).
 
-  #[local] Definition lock' γ_lock :=
-    excl γ_lock ().
-  #[local] Definition lock γ :=
-    lock' γ.(metadata_lock).
+  #[local] Definition owner₁' γ_owner γ_model stable back priv ws : iProp Σ :=
+    twins_twin1 (twins_G := inf_ws_queue_1_G_owner_G) γ_owner (DfracOwn 1) (stable, back, priv) ∗
+    auth_twins_auth _ γ_model ws.
+  #[local] Definition owner₁ γ :=
+    owner₁' γ.(metadata_owner) γ.(metadata_model).
+  #[local] Instance : CustomIpatFormat "owner₁" :=
+    "(
+      Howner₁{} &
+      Hmodel_auth{}
+    )".
+  #[local] Definition owner₂' γ_owner stable back priv :=
+    twins_twin2 (twins_G := inf_ws_queue_1_G_owner_G) γ_owner (stable, back, priv).
+  #[local] Definition owner₂ γ :=
+    owner₂' γ.(metadata_owner).
 
-  #[local] Definition winner₁' γ_winner front Φ :=
-    twins_twin2 (twins_G := inf_ws_queue_1_G_winner_G) γ_winner (front, Next ∘ Φ).
-  #[local] Definition winner₁ γ front Φ :=
-    winner₁' γ.(metadata_winner) front Φ.
-  #[local] Definition winner₂' γ_winner front Φ :=
-    twins_twin1 (twins_G := inf_ws_queue_1_G_winner_G) γ_winner (DfracOwn 1) (front, Next ∘ Φ).
-  #[local] Definition winner₂ γ front Φ :=
-    winner₂' γ.(metadata_winner) front Φ.
-  #[local] Definition winner' γ_winner : iProp Σ :=
-    ∃ front Φ1 Φ2,
-    winner₁' γ_winner front Φ1 ∗
-    winner₂' γ_winner front Φ2.
+  #[local] Definition front_auth' γ_front :=
+    auth_nat_max_auth γ_front (DfracOwn 1).
+  #[local] Definition front_auth γ :=
+    front_auth' γ.(metadata_front).
+  #[local] Definition front_lb γ :=
+    auth_nat_max_lb γ.(metadata_front).
+
+  #[local] Definition history_auth' γ_history :=
+    mono_list_auth γ_history (DfracOwn 1).
+  #[local] Definition history_auth γ :=
+    history_auth' γ.(metadata_history).
+  #[local] Definition history_at γ :=
+    mono_list_at γ.(metadata_history).
+
+  #[local] Definition winner_pop' γ_winner front P : iProp Σ :=
+    twins_twin1 γ_winner (DfracOwn 1) (front, Next P).
+  #[local] Definition winner_pop γ :=
+    winner_pop' γ.(metadata_winner).
+  #[local] Definition winner_steal' γ_winner front P :=
+    twins_twin2 γ_winner (front, Next P).
+  #[local] Definition winner_steal γ :=
+    winner_steal' γ.(metadata_winner).
   #[local] Definition winner γ : iProp Σ :=
-    ∃ front Φ1 Φ2,
-    winner₁ γ front Φ1 ∗
-    winner₂ γ front Φ2.
+    ∃ front P1 P2,
+    winner_pop γ front P1 ∗
+    winner_steal γ front P2.
+  #[local] Instance : CustomIpatFormat "winner" :=
+    "(
+      %front{} &
+      %P1 &
+      %P2 &
+      Hwinner_pop{_{}} &
+      Hwinner_steal{_{}}
+    )".
+
+  #[local] Definition au γ front P : iProp Σ :=
+    AU <{
+      ∃∃ vs,
+      model₁ γ vs
+    }> @ ⊤ ∖ ↑γ.(metadata_inv), ∅ <{
+      ∀∀ v vs',
+      ⌜vs = v :: vs'⌝ ∗
+      model₁ γ vs' ∗
+      history_at γ front v
+    , COMM
+      P
+    }>.
+
+  #[local] Definition inv_state_empty γ stable front back hist lhist : iProp Σ :=
+    ⌜stable = Stable⌝ ∗
+    ⌜front = back⌝ ∗
+    ⌜lhist = hist⌝ ∗
+    ⌜length hist = front⌝ ∗
+    winner γ.
+  #[local] Instance : CustomIpatFormat "inv_state_empty" :=
+    "(
+      {{lazy}{>}%Hstate{}={lazy}%Hstate{}={lazy}%Hstate={>}->=->} &
+      {>=}-> &
+      {>=}-> &
+      {>=}%Hhist{} &
+      Hwinner
+    )".
+  #[local] Definition inv_state_nonempty γ stable front back hist lhist vs prophs : iProp Σ :=
+    ⌜stable = Stable⌝ ∗
+    ⌜front < back⌝ ∗
+    ⌜lhist = hist ++ take 1 vs⌝ ∗
+    ⌜length hist = front⌝ ∗
+    ( winner γ
+    ∨ match prophs with
+      | [] =>
+          False
+      | id :: _ =>
+          ∃ P,
+          identifier_model' id ∗
+          winner_steal γ front P ∗
+          au γ front P
+      end
+    ).
+  #[local] Instance : CustomIpatFormat "inv_state_nonempty" :=
+    "(
+      {{lazy}{>}%Hstate{}={lazy}%Hstate{}={lazy}%Hstate={>}->=->} &
+      {>=}% &
+      {>=}-> &
+      {>=}%Hhist{} &
+      Hwinner
+    )".
+  #[local] Definition inv_state_nonempty_steal γ stable front back hist lhist vs prophs P : iProp Σ :=
+    ⌜stable = Stable⌝ ∗
+    ⌜front < back⌝ ∗
+    ⌜lhist = hist ++ take 1 vs⌝ ∗
+    ⌜length hist = front⌝ ∗
+    match prophs with
+    | [] =>
+        False
+    | id :: _ =>
+        identifier_model' id ∗
+        winner_steal γ front P ∗
+        au γ front P
+    end.
+  #[local] Instance : CustomIpatFormat "inv_state_nonempty_steal" :=
+    "(
+      {{lazy}{>}%Hstate{}={lazy}%Hstate{}={lazy}%Hstate={>}->=->} &
+      {>=}% &
+      {>=}-> &
+      {>=}%Hhist{} &
+      Hid &
+      Hwinner_steal &
+      HP
+    )".
+  #[local] Definition inv_state_emptyish γ stable front back hist lhist prophs : iProp Σ :=
+    ∃ P,
+    ⌜stable = Unstable⌝ ∗
+    ⌜front = back⌝ ∗
+    ⌜lhist = hist⌝ ∗
+    ⌜length hist = S front⌝ ∗
+    ( winner_pop γ front P
+    ∨ winner_steal γ front P ∗
+      P
+    ).
+  #[local] Instance : CustomIpatFormat "inv_state_emptyish" :=
+    "(
+      %P_ &
+      {{lazy}{>}%Hstate{}={lazy}%Hstate{}={lazy}%Hstate={>}->=->} &
+      {>=}-> &
+      {>=}-> &
+      {>=}%Hhist{} &
+      Hwinner
+    )".
+  #[local] Definition inv_state_emptyish_pop γ stable front back hist lhist P : iProp Σ :=
+    ⌜stable = Unstable⌝ ∗
+    ⌜front = back⌝ ∗
+    ⌜lhist = hist⌝ ∗
+    ⌜length hist = S front⌝ ∗
+    winner_pop γ front P.
+  #[local] Instance : CustomIpatFormat "inv_state_emptyish_pop" :=
+    "(
+      {{lazy}{>}%Hstate{}={lazy}%Hstate{}={lazy}%Hstate={>}->=->} &
+      {>=}-> &
+      {>=}-> &
+      {>=}%Hhist{} &
+      Hwinner_pop
+    )".
+  #[local] Definition inv_state_emptyish_steal γ stable front back hist lhist P : iProp Σ :=
+    ⌜stable = Unstable⌝ ∗
+    ⌜front = back⌝ ∗
+    ⌜lhist = hist⌝ ∗
+    ⌜length hist = S front⌝ ∗
+    winner_steal γ front P ∗
+    P.
+  #[local] Instance : CustomIpatFormat "inv_state_emptyish_steal" :=
+    "(
+      {{lazy}{>}%Hstate{}={lazy}%Hstate{}={lazy}%Hstate={>}->=->} &
+      {>=}-> &
+      {>=}-> &
+      {>=}%Hhist{} &
+      Hwinner_steal &
+      HP
+    )".
+  #[local] Definition inv_state_superempty γ stable front back hist lhist : iProp Σ :=
+    ⌜stable = Unstable⌝ ∗
+    ⌜front = S back⌝ ∗
+    ⌜lhist = hist⌝ ∗
+    ⌜length hist = front⌝ ∗
+    winner γ.
+  #[local] Instance : CustomIpatFormat "inv_state_superempty" :=
+    "(
+      {{lazy}{>}%Hstate{}={lazy}%Hstate{}={lazy}%Hstate={>}->=->} &
+      {>=}-> &
+      {>=}-> &
+      {>=}%Hhist{} &
+      Hwinner
+    )".
+  #[local] Definition inv_state γ state stable front back hist lhist vs prophs : iProp Σ :=
+    match state with
+    | Empty =>
+        inv_state_empty γ stable front back hist lhist
+    | Nonempty =>
+        inv_state_nonempty γ stable front back hist lhist vs prophs
+    | Emptyish =>
+        inv_state_emptyish γ stable front back hist lhist prophs
+    | Superempty =>
+        inv_state_superempty γ stable front back hist lhist
+    end.
+
+  #[local] Definition inv_inner l γ : iProp Σ :=
+    ∃ state stable front back hist lhist vs priv pasts prophss,
+    l.[front] ↦ #front ∗
+    l.[back] ↦ #back ∗
+    owner₂ γ stable back priv ∗
+    front_auth γ front ∗
+    ⌜0 < front⌝ ∗
+    model₂ γ vs ∗
+    ⌜length vs = back - front⌝ ∗
+    inf_array_model' γ.(metadata_data) (hist ++ vs) priv ∗
+    history_auth γ lhist ∗
+    wise_prophets_model prophet γ.(metadata_prophet) γ.(metadata_prophet_name) pasts prophss ∗
+    ⌜∀ i, front ≤ i → pasts i = []⌝ ∗
+    inv_state γ state stable front back hist lhist vs (prophss front).
+  #[local] Instance : CustomIpatFormat "inv_inner" :=
+    "(
+      %state{} &
+      %stable{} &
+      %front{} &
+      %back{} &
+      %hist{} &
+      %lhist{} &
+      %vs{} &
+      %priv{} &
+      %pasts{} &
+      %prophss{} &
+      >Hl_front &
+      >Hl_back &
+      >Howner₂ &
+      >Hfront_auth &
+      >%Hfront{} &
+      >Hmodel₂ &
+      >%Hvs{} &
+      >Hdata_model &
+      >Hhistory_auth &
+      >Hprophet_model &
+      >%Hpasts{} &
+      Hstate
+    )".
+  #[local] Definition inv' l γ :=
+    inv γ.(metadata_inv) (inv_inner l γ).
+  Definition inf_ws_queue_1_inv t ι : iProp Σ :=
+    ∃ l γ,
+    ⌜t = #l⌝ ∗
+    ⌜ι = γ.(metadata_inv)⌝ ∗
+    meta l nroot γ ∗
+    l.[data] ↦□ γ.(metadata_data) ∗
+    l.[proph] ↦□ #γ.(metadata_prophet) ∗
+    inf_array_inv γ.(metadata_data) ∗
+    inv' l γ.
+  #[local] Instance : CustomIpatFormat "inv" :=
+    "(
+      %l &
+      %γ &
+      -> &
+      -> &
+      #Hmeta &
+      #Hl_data &
+      #Hl_proph &
+      #Hdata_inv &
+      #Hinv
+    )".
 
   Definition inf_ws_queue_1_model t vs : iProp Σ :=
     ∃ l γ,
     ⌜t = #l⌝ ∗
-    (* metadata *)
     meta l nroot γ ∗
-    (* model values *)
-    model₂ γ vs.
+    model₁ γ vs.
+  #[local] Instance : CustomIpatFormat "model" :=
+    "(
+      %l_ &
+      %γ_ &
+      %Heq &
+      Hmeta_ &
+      Hmodel₁
+    )".
 
-  Definition inf_ws_queue_1_owner t : iProp Σ :=
+  Definition inf_ws_queue_1_owner t ws : iProp Σ :=
     ∃ l γ back priv,
     ⌜t = #l⌝ ∗
-    (* metadata *)
     meta l nroot γ ∗
-    (* control token *)
-    clt₂ γ back priv ∗
-    (* lock *)
-    lock γ.
-
-  #[local] Definition au γ ι Φ : iProp Σ :=
-    AU <{
-      ∃∃ vs,
-      model₂ γ vs
-    }> @ ⊤ ∖ ↑ι, ∅ <{
-      ∀∀ v vs',
-      ⌜vs = v :: vs'⌝ ∗ model₂ γ vs',
-      COMM Φ ‘Some( v )%V
-    }>.
-  #[local] Definition state_inner₁ γ :=
-    winner γ.
-  #[local] Definition state₁ γ front back hist : iProp Σ :=
-    (* physical configuration *)
-    ⌜⁺front = back⌝ ∗
-    (* history values *)
-    history_auth γ hist ∗
-    ⌜length hist = front⌝ ∗
-    (* inner state *)
-    state_inner₁ γ.
-  #[local] Definition state_inner₂ γ ι front prophs : iProp Σ :=
-    match head $ filter (λ '(front', _), front' = front) prophs with
-    | None =>
-        winner γ
-    | Some (_, id) =>
-          winner γ
-        ∨ identifier_model' id ∗
-          ∃ Φ,
-          winner₁ γ front Φ ∗
-          au γ ι Φ
-    end.
-  #[local] Definition state₂ γ ι front back hist vs prophs : iProp Σ :=
-    (* physical configuration *)
-    ⌜(front < back)%Z⌝ ∗
-    (* history values *)
-    history_auth γ (hist ++ [vs !!! 0]) ∗
-    ⌜length hist = front⌝ ∗
-    (* inner state *)
-    state_inner₂ γ ι front prophs.
-  #[local] Definition state_inner₃₁ γ front hist prophs : iProp Σ :=
-    match head $ filter (λ '(front', _), front' = front) prophs with
-    | None =>
-        ∃ Φ,
-        winner₂ γ front Φ
-    | _ =>
-        ∃ Φ,
-        winner₁ γ front Φ ∗
-        Φ ‘Some( hist !!! front )%V
-    end.
-  #[local] Definition state₃₁ γ front back hist prophs : iProp Σ :=
-    (* physical configuration *)
-    ⌜⁺front = back⌝ ∗
-    (* history values *)
-    history_auth γ hist ∗
-    ⌜length hist = S front⌝ ∗
-    (* inner state *)
-    state_inner₃₁ γ front hist prophs.
-  #[local] Definition state_inner₃₂ γ :=
-    winner γ.
-  #[local] Definition state₃₂ γ front back hist : iProp Σ :=
-    (* physical configuration *)
-    ⌜⁺front = (back + 1)%Z⌝ ∗
-    (* history values *)
-    history_auth γ hist ∗
-    ⌜length hist = front⌝ ∗
-    (* inner state *)
-    state_inner₃₂ γ.
-  #[local] Definition state₃ γ front back hist prophs : iProp Σ :=
-    lock γ ∗
-    ( state₃₁ γ front back hist prophs
-    ∨ state₃₂ γ front back hist
-    ).
-  #[local] Definition state γ ι front back hist vs prophs : iProp Σ :=
-      state₁ γ front back hist
-    ∨ state₂ γ ι front back hist vs prophs
-    ∨ state₃ γ front back hist prophs.
-  #[local] Typeclasses Opaque state_inner₁.
-  #[local] Typeclasses Opaque state_inner₂.
-  #[local] Typeclasses Opaque state_inner₃₁.
-  #[local] Typeclasses Opaque state_inner₃₂.
-  #[local] Typeclasses Opaque state.
-  #[local] Ltac unfold_state :=
-    rewrite
-      /state
-      /state_inner₁
-      /state_inner₂
-      /state_inner₃₁
-      /state_inner₃₂.
-
-  #[local] Definition inv_inner l γ ι : iProp Σ :=
-    ∃ front back hist vs priv past prophs,
-    (* mutable physical fields *)
-    l.[front] ↦ #front ∗
-    l.[back] ↦ #back ∗
-    (* control token *)
-    clt₁ γ back priv ∗
-    (* front authority *)
-    front_auth γ front ∗
-    (* data model *)
-    inf_array_model' γ.(metadata_data) (hist ++ vs) priv ∗
-    (* model values *)
-    model₁ γ vs ∗
-    ⌜length vs = ₊(back - front)⌝ ∗
-    (* prophet model *)
-    wise_prophet_model prophet γ.(metadata_prophet) γ.(metadata_prophet_name) past prophs ∗
-    ⌜Forall (λ '(front', _), front' < front) past⌝ ∗
-    (* state *)
-    state γ ι front back hist vs prophs.
-  Definition inf_ws_queue_1_inv t ι : iProp Σ :=
-    ∃ l γ,
-    ⌜t = #l⌝ ∗
-    (* metadata *)
-    meta l nroot γ ∗
-    (* immutable physical fields *)
-    l.[data] ↦□ γ.(metadata_data) ∗
-    l.[proph] ↦□ #γ.(metadata_prophet) ∗
-    (* invariants *)
-    inf_array_inv γ.(metadata_data) ∗
-    inv ι (inv_inner l γ ι).
+    owner₁ γ Stable back priv ws.
+  #[local] Instance : CustomIpatFormat "owner" :=
+    "(
+      %l{=_} &
+      %γ{=_} &
+      %back{} &
+      %priv{} &
+      %Heq{} &
+      Hmeta{=_} &
+      Howner₁{}
+    )".
 
   #[global] Instance inf_ws_queue_1_model_timeless t vs :
     Timeless (inf_ws_queue_1_model t vs).
   Proof.
     apply _.
   Qed.
-  #[global] Instance inf_ws_queue_1_owner_timeless t :
-    Timeless (inf_ws_queue_1_owner t).
+  #[global] Instance inf_ws_queue_1_owner_timeless t ws :
+    Timeless (inf_ws_queue_1_owner t ws).
   Proof.
     apply _.
   Qed.
@@ -322,52 +443,136 @@ Section inf_ws_queue_1_G.
     apply _.
   Qed.
 
-  #[local] Lemma clt_alloc :
+  #[local] Lemma model_owner_alloc :
     ⊢ |==>
-      ∃ γ_ctl,
-      clt₁' γ_ctl 0 (λ _, ()%V) ∗
-      clt₂' γ_ctl 0 (λ _, ()%V).
+      ∃ γ_model γ_owner,
+      model₁' γ_model [] ∗
+      model₂' γ_model [] ∗
+      owner₁' γ_owner γ_model Stable 1 (λ _, ()%V) [] ∗
+      owner₂' γ_owner Stable 1 (λ _, ()%V).
   Proof.
-    apply twins_alloc'.
-  Qed.
-  #[local] Lemma clt_agree γ back1 priv1 back2 priv2 :
-    clt₁ γ back1 priv1 -∗
-    clt₂ γ back2 priv2 -∗
-    ⌜back1 = back2 ∧ priv1 = priv2⌝.
-  Proof.
-    iIntros "Hctl₁ Hctl₂".
-    iDestruct (twins_agree with "Hctl₁ Hctl₂") as %(? & ?%functional_extensionality).
+    iMod (auth_twins_alloc _ (auth_twins_G := inf_ws_queue_1_G_model_G)) as "(%γ_model & Hmodel_auth & Hmodel₁ & Hmodel₂)".
+    iMod (twins_alloc' (twins_G := inf_ws_queue_1_G_owner_G) (Stable, 1, λ _, ()%V)) as "(%γ_owner & Howner₁ & Howner₂)".
     iSteps.
   Qed.
-  #[local] Lemma clt_update {γ back1 priv1 back2 priv2} back priv :
-    clt₁ γ back1 priv1 -∗
-    clt₂ γ back2 priv2 ==∗
-      clt₁ γ back priv ∗
-      clt₂ γ back priv.
+  #[local] Lemma model₁_valid γ stable back priv ws vs :
+    owner₁ γ stable back priv ws -∗
+    model₁ γ vs -∗
+    ⌜vs `suffix_of` ws⌝.
   Proof.
-    apply twins_update'.
+    iIntros "(:owner₁) Hmodel₁".
+    iDestruct (auth_twins_valid_1 with "Hmodel_auth Hmodel₁") as %H.
+    rewrite preorder_rtc in H. iSteps.
+  Qed.
+  #[local] Lemma model₂_valid γ stable back priv ws vs :
+    owner₁ γ stable back priv ws -∗
+    model₂ γ vs -∗
+    ⌜vs `suffix_of` ws⌝.
+  Proof.
+    iIntros "(:owner₁) Hmodel₁".
+    iDestruct (auth_twins_valid_2 with "Hmodel_auth Hmodel₁") as %H.
+    rewrite preorder_rtc in H. iSteps.
+  Qed.
+  #[local] Lemma model_agree γ vs1 vs2 :
+    model₁ γ vs1 -∗
+    model₂ γ vs2 -∗
+    ⌜vs1 = vs2⌝.
+  Proof.
+    apply: auth_twins_agree_L.
+  Qed.
+  #[local] Lemma model_empty {γ stable back priv ws vs1 vs2} :
+    owner₁ γ stable back priv ws -∗
+    model₁ γ vs1 -∗
+    model₂ γ vs2 ==∗
+      owner₁ γ stable back priv [] ∗
+      model₁ γ [] ∗
+      model₂ γ [].
+  Proof.
+    iIntros "(:owner₁) Hmodel₁ Hmodel₂".
+    iMod (auth_twins_update_auth with "Hmodel_auth Hmodel₁ Hmodel₂") as "(Hmodel_auth & Hmodel₁ & Hmodel₂)".
+    iSteps.
+  Qed.
+  #[local] Lemma model_push {γ stable back priv ws vs1 vs2} v :
+    owner₁ γ stable back priv ws -∗
+    model₁ γ vs1 -∗
+    model₂ γ vs2 ==∗
+      owner₁ γ stable back priv (vs1 ++ [v]) ∗
+      model₁ γ (vs1 ++ [v]) ∗
+      model₂ γ (vs1 ++ [v]).
+  Proof.
+    iIntros "(:owner₁) Hmodel₁ Hmodel₂".
+    iMod (auth_twins_update_auth with "Hmodel_auth Hmodel₁ Hmodel₂") as "(Hmodel_auth & Hmodel₁ & Hmodel₂)".
+    iSteps.
+  Qed.
+  #[local] Lemma model_steal γ vs1 vs2 :
+    model₁ γ vs1 -∗
+    model₂ γ vs2 ==∗
+      model₁ γ (tail vs1) ∗
+      model₂ γ (tail vs1).
+  Proof.
+    apply: auth_twins_update_twins_L.
+    rewrite preorder_rtc. apply suffix_tail. done.
+  Qed.
+  #[local] Lemma model_pop γ stable back priv ws vs1 vs2 :
+    owner₁ γ stable back priv ws -∗
+    model₁ γ vs1 -∗
+    model₂ γ vs2 ==∗
+      owner₁ γ stable back priv (removelast vs1) ∗
+      model₁ γ (removelast vs1) ∗
+      model₂ γ (removelast vs1).
+  Proof.
+    iIntros "(:owner₁) Hmodel₁ Hmodel₂".
+    iMod (auth_twins_update_auth with "Hmodel_auth Hmodel₁ Hmodel₂") as "(Hmodel_auth & Hmodel₁ & Hmodel₂)".
+    iSteps.
+  Qed.
+  #[local] Lemma model_pop' γ stable back priv ws vs1 v vs2 :
+    owner₁ γ stable back priv ws -∗
+    model₁ γ (vs1 ++ [v]) -∗
+    model₂ γ vs2 ==∗
+      owner₁ γ stable back priv vs1 ∗
+      model₁ γ vs1 ∗
+      model₂ γ vs1.
+  Proof.
+    rewrite -{2 3 4}(removelast_last vs1 v).
+    apply model_pop.
+  Qed.
+
+  #[local] Lemma owner₁_exclusive γ stable1 back1 priv1 ws1 stable2 back2 priv2 ws2 :
+    owner₁ γ stable1 back1 priv1 ws1 -∗
+    owner₁ γ stable2 back2 priv2 ws2 -∗
+    False.
+  Proof.
+    iIntros "(:owner₁ =1) (:owner₁ =2)".
+    iApply (twins_twin1_exclusive with "Howner₁1 Howner₁2").
+  Qed.
+  #[local] Lemma owner_agree γ stable1 back1 priv1 ws stable2 back2 priv2 :
+    owner₁ γ stable1 back1 priv1 ws -∗
+    owner₂ γ stable2 back2 priv2 -∗
+      ⌜stable1 = stable2⌝ ∗
+      ⌜back1 = back2⌝ ∗
+      ⌜priv1 = priv2⌝.
+  Proof.
+    iIntros "(:owner₁) Howner₂".
+    iDestruct (twins_agree_L with "Howner₁ Howner₂") as %[= <- <- <-].
+    iSteps.
+  Qed.
+  #[local] Lemma owner_update {γ stable1 back1 priv1 ws stable2 back2 priv2} stable back priv :
+    owner₁ γ stable1 back1 priv1 ws -∗
+    owner₂ γ stable2 back2 priv2 ==∗
+      owner₁ γ stable back priv ws ∗
+      owner₂ γ stable back priv.
+  Proof.
+    iIntros "(:owner₁) Howner₂".
+    iMod (twins_update' with "Howner₁ Howner₂") as "(Howner₁ & Howner₂)".
+    iSteps.
   Qed.
 
   #[local] Lemma front_alloc :
     ⊢ |==>
       ∃ γ_front,
-      front_auth' γ_front 0.
+      front_auth' γ_front 1.
   Proof.
     apply auth_nat_max_alloc.
-  Qed.
-  #[local] Lemma front_valid γ front1 front2 :
-    front_auth γ front1 -∗
-    front_lb γ front2 -∗
-    ⌜front2 ≤ front1⌝.
-  Proof.
-    apply auth_nat_max_lb_valid.
-  Qed.
-  #[local] Lemma front_auth_update {γ front} front' :
-    front ≤ front' →
-    front_auth γ front ⊢ |==>
-    front_auth γ front'.
-  Proof.
-    apply auth_nat_max_update.
   Qed.
   #[local] Lemma front_lb_get γ front :
     front_auth γ front ⊢
@@ -382,44 +587,48 @@ Section inf_ws_queue_1_G.
   Proof.
     apply auth_nat_max_lb_le.
   Qed.
-  #[local] Lemma front_state₃₂ γ ι front front' back hist vs prophs :
-    back = (front' - 1)%Z →
-    front_auth γ front -∗
-    front_lb γ front' -∗
-    state γ ι front back hist vs prophs -∗
-      ⌜front = front'⌝ ∗
-      front_auth γ front' ∗
-      lock γ ∗
-      state₃₂ γ front' back hist.
+  #[local] Lemma front_lb_valid γ front1 front2 :
+    front_auth γ front1 -∗
+    front_lb γ front2 -∗
+    ⌜front2 ≤ front1⌝.
   Proof.
-    iIntros (->) "Hfront_auth #Hfront_lb Hstate".
-    iDestruct (front_valid with "Hfront_auth Hfront_lb") as %Hle.
-    unfold_state. iDestruct "Hstate" as "[Hstate | [Hstate | (Hlock & [Hstate | Hstate])]]";
-      iDestruct "Hstate" as "(%Hstate & Hhist_auth & %Hhist & Hstate)";
-      [lia.. |].
-    assert (front' = front) as -> by lia. iSteps.
+    apply auth_nat_max_lb_valid.
+  Qed.
+  #[local] Lemma front_update γ front :
+    front_auth γ front ⊢ |==>
+    front_auth γ (S front).
+  Proof.
+    apply auth_nat_max_update; first lia.
   Qed.
 
   #[local] Lemma history_alloc :
     ⊢ |==>
-      ∃ γ_history,
-      history_auth' γ_history [].
+      ∃ γ_hist,
+      history_auth' γ_hist [()%V].
   Proof.
     apply mono_list_alloc.
   Qed.
-  #[local] Lemma history_at_get {γ hist} i v :
-    hist !! i = Some v →
-    history_auth γ hist ⊢
+  #[local] Lemma history_at_get {γ hist v} i :
+    i = length hist →
+    history_auth γ (hist ++ [v]) ⊢
     history_at γ i v.
   Proof.
-    apply mono_list_at_get.
+    intros ->.
+    apply mono_list_at_get, list_lookup_middle. done.
   Qed.
-  #[local] Lemma history_agree γ hist i v :
+  #[local] Lemma history_at_lookup γ hist i v :
     history_auth γ hist -∗
     history_at γ i v -∗
     ⌜hist !! i = Some v⌝.
   Proof.
     apply mono_list_at_valid.
+  Qed.
+  #[local] Lemma history_at_agree γ i v1 v2 :
+    history_at γ i v1 -∗
+    history_at γ i v2 -∗
+    ⌜v1 = v2⌝.
+  Proof.
+    apply mono_list_at_agree.
   Qed.
   #[local] Lemma history_update {γ hist} v :
     history_auth γ hist ⊢ |==>
@@ -428,451 +637,201 @@ Section inf_ws_queue_1_G.
     apply mono_list_update_snoc.
   Qed.
 
-  #[local] Lemma model_alloc :
-    ⊢ |==>
-      ∃ γ_model,
-      model₁' γ_model [] ∗
-      model₂' γ_model [].
-  Proof.
-    iMod (twins_alloc' (twins_G := inf_ws_queue_1_G_model_G) []) as "(%γ_model & Hmodel₁ & Hmodel₂)".
-    iSteps.
-  Qed.
-  #[local] Lemma model_agree γ vs1 vs2 :
-    model₁ γ vs1 -∗
-    model₂ γ vs2 -∗
-    ⌜vs1 = vs2⌝.
-  Proof.
-    iIntros "Hmodel₁ Hmodel₂".
-    iDestruct (twins_agree_L with "Hmodel₂ Hmodel₁") as %->.
-    iSteps.
-  Qed.
-  #[local] Lemma model_update {γ vs1 vs2} vs :
-    model₁ γ vs1 -∗
-    model₂ γ vs2 ==∗
-      model₁ γ vs ∗
-      model₂ γ vs.
-  Proof.
-    iIntros "Hmodel₁ Hmodel₂".
-    iMod (twins_update' with "Hmodel₂ Hmodel₁") as "(Hmodel₂ & Hmodel₁)".
-    iSteps.
-  Qed.
-
-  #[local] Lemma lock_alloc :
-    ⊢ |==>
-      ∃ γ_lock,
-      lock' γ_lock.
-  Proof.
-    apply excl_alloc.
-  Qed.
-  #[local] Lemma lock_exclusive γ :
-    lock γ -∗
-    lock γ -∗
-    False.
-  Proof.
-    apply excl_exclusive.
-  Qed.
-  #[local] Lemma lock_state γ ι front back hist vs prophs :
-    lock γ -∗
-    state γ ι front back hist vs prophs -∗
-      lock γ ∗
-      ( state₁ γ front back hist
-      ∨ state₂ γ ι front back hist vs prophs
-      ).
-  Proof.
-    unfold_state. iIntros "Hlock [Hstate | [Hstate | (Hlock' & Hstate)]]"; [iFrame.. |].
-    iDestruct (lock_exclusive with "Hlock Hlock'") as %[].
-  Qed.
-
   #[local] Lemma winner_alloc :
     ⊢ |==>
       ∃ γ_winner,
-      winner' γ_winner.
+      winner_pop' γ_winner 1 True ∗
+      winner_steal' γ_winner 1 True.
   Proof.
-    iMod (twins_alloc' (twins_G := inf_ws_queue_1_G_winner_G) (inhabitant, λ _, Next inhabitant)) as "(%γ_winner & Hwinner₁ & Hwinner₂)".
-    iSteps.
+    apply twins_alloc'.
   Qed.
-  #[local] Lemma winner₁_exclusive γ front1 Φ1 front2 Φ2 :
-    winner₁ γ front1 Φ1 -∗
-    winner₁ γ front2 Φ2 -∗
-    False.
-  Proof.
-    apply twins_twin2_exclusive.
-  Qed.
-  #[local] Lemma winner₁_exclusive' γ front Φ :
-    winner₁ γ front Φ -∗
-    winner γ -∗
-    False.
-  Proof.
-    iIntros "Hwinner₁ (%front' & %Φ1 & %Φ2 & Hwinner₁' & Hwinner₂)".
-    iApply (winner₁_exclusive with "Hwinner₁ Hwinner₁'").
-  Qed.
-  #[local] Lemma winner₂_exclusive γ front1 Φ1 front2 Φ2 :
-    winner₂ γ front1 Φ1 -∗
-    winner₂ γ front2 Φ2 -∗
+  #[local] Lemma winner_pop_exclusive γ front1 P1 front2 P2 :
+    winner_pop γ front1 P1 -∗
+    winner_pop γ front2 P2 -∗
     False.
   Proof.
     apply twins_twin1_exclusive.
   Qed.
-  #[local] Lemma winner₂_exclusive' γ front Φ :
-    winner₂ γ front Φ -∗
+  #[local] Lemma winner_pop_exclusive' γ front P :
+    winner_pop γ front P -∗
     winner γ -∗
     False.
   Proof.
-    iIntros "Hwinner₂ (%front' & %Φ1 & %Φ2 & Hwinner₁ & Hwinner₂')".
-    iApply (winner₂_exclusive with "Hwinner₂ Hwinner₂'").
+    iIntros "Hwinner_pop_1 (:winner =2)".
+    iApply (winner_pop_exclusive with "Hwinner_pop_1 Hwinner_pop_2").
   Qed.
-  #[local] Lemma winner_agree {γ front1 Φ1 front2 Φ2} v :
-    winner₁ γ front1 Φ1 -∗
-    winner₂ γ front2 Φ2 -∗
-      ⌜front1 = front2⌝ ∗
-      ▷ (Φ1 v ≡ Φ2 v) ∗
-      winner₁ γ front1 Φ1 ∗
-      winner₂ γ front1 Φ2.
-  Proof.
-    iIntros "Hwinner₁ Hwinner₂".
-    iDestruct (twins_agree with "Hwinner₂ Hwinner₁") as "#HΦ".
-    rewrite prod_equivI /=. iDestruct "HΦ" as "(% & HΦ)". simplify.
-    iFrame. iSplit; first iSteps.
-    rewrite discrete_fun_equivI. iDestruct ("HΦ" $! v) as "HΦv". rewrite later_equivI.
-    iModIntro. iRewrite "HΦv". iSteps.
-  Qed.
-  #[local] Lemma winner_update {γ front1 Φ1 front2 Φ2} front Φ :
-    winner₁ γ front1 Φ1 -∗
-    winner₂ γ front2 Φ2 ==∗
-      winner₁ γ front Φ ∗
-      winner₂ γ front Φ.
-  Proof.
-    iIntros "Hwinner₁ Hwinner₂".
-    iMod (twins_update (twins_G := inf_ws_queue_1_G_winner_G) (front, Next ∘ Φ) with "Hwinner₂ Hwinner₁") as "($ & $)"; first done.
-    iSteps.
-  Qed.
-  #[local] Lemma winner₁_state γ ι front front' back hist vs prophs Φ :
-    winner₁ γ front Φ -∗
-    state γ ι front' back hist vs prophs -∗
-      ⌜front' = front⌝ ∗
-      ⌜back = front⌝ ∗
-      lock γ ∗
-      history_auth γ hist ∗
-      ⌜length hist = S front⌝ ∗
-        ∃ Φ',
-        ⌜head $ filter (λ '(front', _), front' = front) prophs = None⌝ ∗
-        winner₁ γ front Φ ∗
-        winner₂ γ front Φ'.
-  Proof.
-    unfold_state. iIntros "Hwinner₁ [Hstate | [Hstate | Hstate]]".
-    - iDestruct "Hstate" as "(_ & _ & _ & Hstate)".
-      iDestruct (winner₁_exclusive' with "Hwinner₁ Hstate") as %[].
-    - iDestruct "Hstate" as "(_ & _ & _ & Hstate)".
-      unfold_state. destruct (head $ filter _ _) as [(_front' & id) |].
-      + iDestruct "Hstate" as "[Hstate | (_ & % & Hwinner₁' & _)]".
-        * iDestruct (winner₁_exclusive' with "Hwinner₁ Hstate") as %[].
-        * iDestruct (winner₁_exclusive with "Hwinner₁ Hwinner₁'") as %[].
-      + iDestruct (winner₁_exclusive' with "Hwinner₁ Hstate") as %[].
-    - iDestruct "Hstate" as "(Hlock & [(<- & Hhist_auth & -> & Hstate) | (_ & _ & _ & Hstate)])".
-      + unfold_state. destruct (head $ filter _ _) as [proph |] eqn:Hprophs.
-        * iDestruct "Hstate" as "(% & Hwinner₁' & _)".
-          iDestruct (winner₁_exclusive with "Hwinner₁ Hwinner₁'") as %[].
-        * iDestruct "Hstate" as "(%Φ' & Hwinner₂)".
-          iDestruct (winner_agree inhabitant with "Hwinner₁ Hwinner₂") as "(<- & _ & Hwinner₁ & Hwinner₂)".
-          iSteps.
-      + iDestruct (winner₁_exclusive' with "Hwinner₁ Hstate") as %[].
-  Qed.
-  #[local] Lemma winner₂_state γ ι front front' back hist vs prophs Φ :
-    winner₂ γ front Φ -∗
-    state γ ι front' back hist vs prophs -∗
-      ⌜front' = front⌝ ∗
-      ( ⌜(front < back)%Z⌝ ∗
-        history_auth γ (hist ++ [vs !!! 0]) ∗
-        ⌜length hist = front⌝ ∗
-        ( ∃ id Φ',
-          ⌜head $ filter (λ '(front', _), front' = front) prophs = Some (front, id)⌝ ∗
-          winner₁ γ front Φ' ∗
-          winner₂ γ front Φ ∗
-          identifier_model' id ∗
-          au γ ι Φ'
-        )
-      ∨ ⌜back = front⌝ ∗
-        lock γ ∗
-        history_auth γ hist ∗
-        ⌜length hist = S front⌝ ∗
-        ( ∃ id Φ',
-          ⌜head $ filter (λ '(front', _), front' = front) prophs = Some (front, id)⌝ ∗
-          winner₁ γ front Φ' ∗
-          winner₂ γ front Φ ∗
-          Φ' ‘Some( hist !!! front )%V
-        )
-      ).
-  Proof.
-    unfold_state. iIntros "Hwinner₂ [Hstate | [Hstate | Hstate]]".
-    - iDestruct "Hstate" as "(_ & _ & _ & Hstate)".
-      iDestruct (winner₂_exclusive' with "Hwinner₂ Hstate") as %[].
-    - iDestruct "Hstate" as "(%Hstate & Hhist_auth & -> & Hstate)".
-      unfold_state. destruct (head $ filter _ _) as [(_front' & id) |] eqn:Hprophs.
-      + iDestruct "Hstate" as "[Hstate | (Hid & %Φ' & Hwinner₁ & HΦ')]".
-        * iDestruct (winner₂_exclusive' with "Hwinner₂ Hstate") as %[].
-        * iDestruct (winner_agree inhabitant with "Hwinner₁ Hwinner₂") as "(-> & _ & Hwinner₁ & Hwinner₂)".
-          pose proof Hprophs as (-> & _)%head_Some_elem_of%elem_of_list_filter. iSteps.
-      + iDestruct (winner₂_exclusive' with "Hwinner₂ Hstate") as %[].
-    - iDestruct "Hstate" as "(Hlock & [(<- & Hhist_auth & -> & Hstate) | (_ & _ & _ & Hstate)])".
-      + unfold_state. destruct (head $ filter _ _) as [(_front' & id) |] eqn:Hprophs.
-        * iDestruct "Hstate" as "(%Φ' & Hwinner₁ & HΦ')".
-          iDestruct (winner_agree inhabitant with "Hwinner₁ Hwinner₂") as "(-> & _ & Hwinner₁ & Hwinner₂)".
-          pose proof Hprophs as (-> & _)%head_Some_elem_of%elem_of_list_filter. iSteps.
-        * iDestruct "Hstate" as "(%Φ' & Hwinner₂')".
-          iDestruct (winner₂_exclusive with "Hwinner₂ Hwinner₂'") as %[].
-      + iDestruct (winner₂_exclusive' with "Hwinner₂ Hstate") as %[].
-  Qed.
-  #[local] Lemma winner₂_state' γ ι front front' hist vs prophs Φ :
-    winner₂ γ front Φ -∗
-    state γ ι front' front hist vs prophs -∗
-      ⌜front' = front⌝ ∗
-      lock γ ∗
-      history_auth γ hist ∗
-      ⌜length hist = S front⌝ ∗
-        ∃ id Φ',
-        ⌜head $ filter (λ '(front', _), front' = front) prophs = Some (front, id)⌝ ∗
-        winner₁ γ front Φ' ∗
-        winner₂ γ front Φ ∗
-        Φ' ‘Some( hist !!! front )%V.
-  Proof.
-    iIntros "Hwinner₂ Hstate".
-    iDestruct (winner₂_state with "Hwinner₂ Hstate") as "($ & [Hstate | Hstate])".
-    - iDestruct "Hstate" as "(%Hstate & _)". lia.
-    - iSteps.
-  Qed.
-
-  Lemma inf_ws_queue_1_owner_exclusive t :
-    inf_ws_queue_1_owner t -∗
-    inf_ws_queue_1_owner t -∗
+  #[local] Lemma winner_steal_exclusive γ front1 P1 front2 P2 :
+    winner_steal γ front1 P1 -∗
+    winner_steal γ front2 P2 -∗
     False.
   Proof.
-    iIntros "(%l & %γ & %back & %priv & -> & #Hmeta & Hctl₂1 & Hlock1) (%_l & %_γ & %_back & %_priv & %Heq & #_Hmeta & Hctl₂2 & Hlock2)". injection Heq as <-.
-    iDestruct (meta_agree with "Hmeta _Hmeta") as %->. iClear "_Hmeta".
-    iApply (lock_exclusive with "Hlock1 Hlock2").
+    apply twins_twin2_exclusive.
+  Qed.
+  #[local] Lemma winner_steal_exclusive' γ front P :
+    winner_steal γ front P -∗
+    winner γ -∗
+    False.
+  Proof.
+    iIntros "Hwinner_steal_1 (:winner =2)".
+    iApply (winner_steal_exclusive with "Hwinner_steal_1 Hwinner_steal_2").
+  Qed.
+  #[local] Lemma winner_agree γ front1 P1 front2 P2 :
+    winner_pop γ front1 P1 -∗
+    winner_steal γ front2 P2 -∗
+      ⌜front1 = front2⌝ ∗
+      ▷ (P1 ≡ P2).
+  Proof.
+    iIntros "Hwinner_pop Hwinner_steal".
+    iDestruct (twins_agree with "Hwinner_pop Hwinner_steal") as "#Heq".
+    rewrite prod_equivI /= discrete_eq_1.
+    iDestruct "Heq" as "($ & $)".
+  Qed.
+  #[local] Lemma winner_update {γ front1 P1 front2 P2} front P :
+    winner_pop γ front1 P1 -∗
+    winner_steal γ front2 P2 ==∗
+      winner_pop γ front P ∗
+      winner_steal γ front P.
+  Proof.
+    apply twins_update'.
   Qed.
 
-  #[local] Lemma inf_array_get_spec_history l γ ι i v :
-    {{{
-      inf_array_inv γ.(metadata_data) ∗
-      inv ι (inv_inner l γ ι) ∗
-      l.[data] ↦□ γ.(metadata_data) ∗
-      history_at γ i v
-    }}}
-      inf_array_get (#l).{data} #i
-    {{{
-      RET v;
-      True
-    }}}.
+  Opaque owner₁'.
+
+  Lemma inf_ws_queue_1_owner_exclusive t ws1 ws2 :
+    inf_ws_queue_1_owner t ws1 -∗
+    inf_ws_queue_1_owner t ws2 -∗
+    False.
   Proof.
-    iIntros "%Φ (#Harray_inv & #Hinv & #Hdata & #Hhist_at) HΦ".
-
-    (* → [!#l.[data]] *)
-    wp_load.
-
-    (* → [array.(inf_array_get) data #i] *)
-    awp_apply (inf_array_get_spec with "Harray_inv") without "HΦ"; first lia.
-    (* open invariant *)
-    iInv "Hinv" as "(%front & %back & %hist & %vs & %priv & %past & %prophs & Hfront & Hback & Hctl₁ & Hfront_auth & >Harray_model & Hmodel₁ & >%Hmodel & Hprophet_model & >%Hpast & Hstate)".
-    (* we have [(hist ++ vs) !! i = Some v] *)
-    iAssert (◇ ⌜(hist ++ vs) !! i = Some v⌝)%I as "#>%Hlookup".
-    { unfold_state. iDestruct "Hstate" as "[Hstate | [Hstate | (_ & [Hstate | Hstate])]]";
-        iDestruct "Hstate" as "(>%Hstate & >Hhist_auth & >%Hhist & _)";
-        iModIntro;
-        iDestruct (history_agree with "Hhist_auth Hhist_at") as %?;
-        iPureIntro.
-      - erewrite lookup_app_l_Some => //.
-      - destruct vs as [| w vs]; simpl in *; first lia.
-        rewrite (assoc (++) hist [w]). erewrite lookup_app_l_Some => //.
-      - rewrite (nil_length_inv vs); first lia. list_simplifier. done.
-      - rewrite (nil_length_inv vs); first lia. erewrite lookup_app_l_Some => //.
-    }
-    iAaccIntro with "Harray_model"; iIntros "Harray_model".
-    { iModIntro. rewrite right_id. repeat iExists _. iFrameSteps. }
-    (* close invariant *)
-    iModIntro. iSplitL.
-    { repeat iExists _. iFrameSteps. }
-    iIntros "_ HΦ".
-    clear- Hlookup.
-
-    rewrite Nat2Z.id decide_True; first eauto using lookup_lt_Some.
-    erewrite list_lookup_total_correct => //.
-    iApply ("HΦ" with "[//]").
+    iIntros "(:owner =1) (:owner =2)". subst t. injection Heq2 as <-.
+    iDestruct (meta_agree with "Hmeta1 Hmeta2") as %<-. iClear "Hmeta2".
+    iApply (owner₁_exclusive with "Howner₁1 Howner₁2").
   Qed.
-  #[local] Lemma inf_array_get_spec_private l γ ι back priv i :
-    (back ≤ i)%Z →
-    {{{
-      inf_array_inv γ.(metadata_data) ∗
-      inv ι (inv_inner l γ ι) ∗
-      l.[data] ↦□ γ.(metadata_data) ∗
-      clt₂ γ back priv ∗
-      lock γ
-    }}}
-      inf_array_get (#l).{data} #i
-    {{{
-      RET priv ₊(i - back);
-      clt₂ γ back priv ∗
-      lock γ
-    }}}.
+  Lemma inf_ws_queue_1_model_valid t ws vs :
+    inf_ws_queue_1_owner t ws -∗
+    inf_ws_queue_1_model t vs -∗
+    ⌜vs `suffix_of` ws⌝.
   Proof.
-    iIntros "%Hi %Φ (#Harray_inv & #Hinv & #Hdata & Hctl₂ & Hlock) HΦ".
-
-    (* → [!#l.[data]] *)
-    wp_load.
-
-    (* open invariant *)
-    iApply fupd_wp. iMod (inv_acc with "Hinv") as "((%front & %_back & %hist & %vs & %_priv & %past & %prophs & Hfront & Hback & >Hctl₁ & Hfront_auth & Harray_model & Hmodel₁ & >%Hmodel & Hprophet_model & >%Hpast & Hstate) & Hclose)"; first done.
-    iDestruct (clt_agree with "Hctl₁ Hctl₂") as %(-> & ->).
-    (* we have [0 ≤ back] *)
-    iAssert (◇ ⌜0 ≤ back⌝)%I%Z as "#>%Hback".
-    { (* we have lock, hence we are in state 1 or in state 2 *)
-      iDestruct (lock_state with "Hlock Hstate") as "(Hlock & [Hstate | Hstate])";
-        iDestruct "Hstate" as "(>%Hstate & _)"; auto with lia.
-    }
-    (* close invariant *)
-    iMod ("Hclose" with "[- Hctl₂ Hlock HΦ]") as "_".
-    { repeat iExists _. iFrame. done. }
-    iModIntro.
-    clear- Hi Hback.
-
-    (* → [array.(inf_array_get) data #i] *)
-    awp_apply (inf_array_get_spec' with "Harray_inv"); first lia.
-    (* open invariant *)
-    iInv "Hinv" as "(%front & %_back & %hist & %vs & %_priv & %past & %prophs & Hfront & Hback & >Hctl₁ & Hfront_auth & >Harray_model & Hmodel₁ & >%Hvs & Hprophet_model & >%Hpast & Hstate)".
-    iDestruct (clt_agree with "Hctl₁ Hctl₂") as %(-> & ->).
-    (* we have [back = length (hist ++ vs)] *)
-    iAssert (◇ ⌜back = length (hist ++ vs)⌝)%I%Z as "#>%Hback'".
-    { (* we have lock, hence we are in state 1 or in state 2 *)
-      iDestruct (lock_state with "Hlock Hstate") as "(Hlock & [Hstate | Hstate])";
-        iDestruct "Hstate" as "(>%Hstate & _ & >%Hhist & _)";
-        simpl_length; auto with lia.
-    }
-    iAaccIntro with "Harray_model"; iIntros "Harray_model".
-    { iModIntro. iFrame. repeat iExists _. iFrame. done. }
-    (* close invariant *)
-    iModIntro. iSplitR "Hctl₂ Hlock HΦ".
-    { repeat iExists _. iFrame. done. }
-    iIntros "_".
-    clear- Hi Hback Hback'.
-
-    rewrite decide_False; first lia.
-    assert (₊i - length (hist ++ vs) = ₊(i - back)) as -> by lia.
-    iApply "HΦ". iFrame.
+    iIntros "(:owner =1) (:model)". subst t. injection Heq as <-.
+    iDestruct (meta_agree with "Hmeta1 Hmeta_") as %<-. iClear "Hmeta_".
+    iApply (model₁_valid with "Howner₁1 Hmodel₁").
   Qed.
 
-  #[local] Lemma wp_resolve_inconsistent_1 l γ ι front id prophs_lb (front1 front2 : Z) :
-    head $ filter (λ '(front', _), front' = front) prophs_lb = None →
-    {{{
-      inf_array_inv γ.(metadata_data) ∗
-      inv ι (inv_inner l γ ι) ∗
-      wise_prophet_lb prophet γ.(metadata_prophet_name) prophs_lb
-    }}}
-      Resolve (CAS (#l).[front]%V #front1 #front2) #γ.(metadata_prophet) (#front, #id)%V
-    {{{ v,
-      RET v; False
-    }}}.
+  #[local] Lemma inv_state_Stable γ state front back hist lhist vs prophs :
+    length vs = back - front →
+    inv_state γ state Stable front back hist lhist vs prophs ⊢
+      ⌜state = Empty ∨ state = Nonempty⌝ ∗
+      ⌜front ≤ back⌝ ∗
+      ⌜length (hist ++ vs) = back⌝.
   Proof.
-    iIntros (Hprophs_lb%head_None) "%Φ (#Harray_inv & #Hinv & #Hprophet_lb) HΦ".
-
-    (* open invariant *)
-    iInv "Hinv" as "(%front' & %back & %hist & %vs & %priv & %past & %prophs & Hfront & Hback & Hctl₁ & Hfront_auth & Harray_model & Hmodel₁ & >%Hvs & >Hprophet_model & >%Hpast & Hstate)".
-    (* current prophecies are a suffix of prophet lower bound *)
-    iDestruct (wise_prophet_lb_valid with "Hprophet_model Hprophet_lb") as %(past1 & past2 & -> & ->).
-    (* do resolve *)
-    wp_apply (wise_prophet_wp_resolve prophet(front, id) with "Hprophet_model"); [done.. |].
-    (* whether CAS succeed or not, we reach a contradiction *)
-    wp_cas as _ | _.
-    all: iModIntro; iIntros "%prophs' ->".
-    all: eelim (filter_nil_not_elem_of _ _ (front, id)); [done.. |].
-    all: apply elem_of_app; right; apply elem_of_cons; naive_solver.
+    iIntros "%Hvs Hstate".
+    rewrite length_app.
+    destruct state.
+    - iDestruct "Hstate" as "(:inv_state_empty lazy=)".
+      iSteps.
+    - iDestruct "Hstate" as "(:inv_state_nonempty lazy=)".
+      iSteps.
+    - iDestruct "Hstate" as "(:inv_state_emptyish lazy=)". done.
+    - iDestruct "Hstate" as "(:inv_state_superempty lazy=)". done.
   Qed.
-  #[local] Lemma wp_resolve_loser l γ ι front _front id id' prophs_lb v :
-    head $ filter (λ '(front', _), front' = front) prophs_lb = Some (_front, id') →
-    id ≠ id' →
-    {{{
-      inf_array_inv γ.(metadata_data) ∗
-      inv ι (inv_inner l γ ι) ∗
-      front_lb γ front ∗
-      wise_prophet_lb prophet γ.(metadata_prophet_name) prophs_lb
-    }}}
-      Resolve (CAS (#l).[front]%V #front v) #γ.(metadata_prophet) (#front, #id)%V
-    {{{
-      RET #false;
-      front_lb γ (S front)
-    }}}.
+  #[local] Lemma inv_state_Unstable γ state front back hist lhist vs prophs :
+    inv_state γ state Unstable front back hist lhist vs prophs ⊢
+      ⌜state = Emptyish ∨ state = Superempty⌝ ∗
+      ⌜front = back ∨ front = S back⌝.
   Proof.
-    iIntros "%Hprophs_lb %Hid %Φ (#Harray_inv & #Hinv & #Hfront_lb & #Hprophet_lb) HΦ".
-
-    (* open invariant *)
-    iInv "Hinv" as "(%front' & %back & %hist & %vs & %priv & %past & %prophs & Hfront & Hback & Hctl₁ & Hfront_auth & Harray_model & Hmodel₁ & >%Hvs & >Hprophet_model & >%Hpast & Hstate)".
-    (* current prophecies are a suffix of prophet lower bound *)
-    iDestruct (wise_prophet_lb_valid with "Hprophet_model Hprophet_lb") as %(past1 & past2 & -> & ->).
-    (* do resolve *)
-    wp_apply (wise_prophet_wp_resolve prophet (front, id) with "Hprophet_model"); [done.. |].
-    (* CAS must fail as we are not the winner: [id ≠ id'] *)
-    wp_cas as _Hfront | ->%val_similar_nat; last first.
-    { iModIntro. iIntros "%prophs' -> Hprophet_model".
-      rewrite filter_app filter_cons_True // in Hprophs_lb.
-      simpl in *. destruct (filter _ past2) as [| (__front & id'')] eqn:Hpast2; first naive_solver.
-      apply (f_equal head), head_Some_elem_of, elem_of_list_filter in Hpast2 as (-> & Hpast2).
-      rewrite Forall_app !Forall_forall in Hpast. naive_solver lia.
-    }
-    iAssert ⌜front < front'⌝%I as %Hfront; last clear _Hfront.
-    { iDestruct (front_valid with "Hfront_auth Hfront_lb") as %?.
-      iPureIntro. assert (front ≠ front') by naive_solver. lia.
-    }
-    iModIntro. iIntros "%prophs' -> Hprophet_model".
-    (* emit front fragment at [S front] *)
-    iClear "Hfront_lb".
-    iDestruct (front_lb_get with "Hfront_auth") as "#_Hfront_lb".
-    iDestruct (front_lb_le (S front) with "_Hfront_lb") as "#Hfront_lb"; first lia.
-    iClear "_Hfront_lb".
-    (* close invariant *)
-    iModIntro. iSplitR "HΦ".
-    { iExists front', back, hist, vs, priv, _, prophs'. iFrame.
-      iSplit; first done.
-      iSplit. { iPureIntro. decompose_Forall; done. }
-      unfold_state. iDestruct "Hstate" as "[Hstate | [(%Hstate & Hstate) | (Hlock & [(%Hstate & Hstate) | Hstate])]]".
-      - iLeft. done.
-      - iRight. iLeft. iFrame. iSplit; first done.
-        unfold_state. rewrite filter_cons_False //. lia.
-      - do 2 iRight. iFrame. iLeft. iFrame. iSplit; first done.
-        unfold_state. rewrite filter_cons_False //. lia.
-      - do 2 iRight. iFrame.
-    }
-    clear.
-
-    iApply ("HΦ" with "Hfront_lb").
+    iIntros "Hstate".
+    destruct state.
+    - iDestruct "Hstate" as "(:inv_state_empty lazy=)". done.
+    - iDestruct "Hstate" as "(:inv_state_nonempty lazy=)". done.
+    - iDestruct "Hstate" as "(:inv_state_emptyish lazy=)".
+      iSteps.
+    - iDestruct "Hstate" as "(:inv_state_superempty lazy=)".
+      iSteps.
   Qed.
-  #[local] Lemma wp_resolve_inconsistent_2 l γ ι front _front priv Ψ id id' prophs_lb v :
-    head $ filter (λ '(front', _), front' = front) prophs_lb = Some (_front, id') →
-    id ≠ id' →
-    {{{
-      inf_array_inv γ.(metadata_data) ∗
-      inv ι (inv_inner l γ ι) ∗
-      clt₂ γ front priv ∗
-      front_lb γ front ∗
-      wise_prophet_lb prophet γ.(metadata_prophet_name) prophs_lb ∗
-      winner₂ γ front Ψ
-    }}}
-      Resolve (CAS (#l).[front]%V #front v) #γ.(metadata_prophet) (#front, #id)%V
-    {{{
-      RET #false; False
-    }}}.
+  #[local] Lemma inv_state_Nonempty γ state stable front back hist lhist vs prophs :
+    front < back →
+    inv_state γ state stable front back hist lhist vs prophs ⊢
+    ⌜state = Nonempty⌝.
   Proof.
-    iIntros "%Hprophs_lb %Hid %Φ (#Harray_inv & #Hinv & Hctl₂ & #Hfront_lb & #Hprophet_lb & Hwinner₂) HΦ".
-
-    (* do resolve *)
-    iApply wp_fupd.
-    wp_apply (wp_resolve_loser with "[$Harray_inv $Hinv $Hfront_lb $Hprophet_lb]"); [done.. |]. iClear "Hfront_lb". iIntros "#Hfront_lb".
-
-    (* open invariant *)
-    iMod (inv_acc with "Hinv") as "((%front' & %_back & %hist & %vs & %_priv & %past & %prophs & Hfront & Hback & >Hctl₁ & >Hfront_auth & Harray_model & Hmodel₁ & >%Hvs & Hprophet_model & >%Hpast & Hstate) & Hclose)"; first done.
-    iDestruct (clt_agree with "Hctl₁ Hctl₂") as "(-> & ->)".
-    (* we are in state 3.1, hence [front' = front] *)
-    iAssert (◇ ⌜front' = front⌝)%I as "#>->".
-    { iDestruct (winner₂_state' with "Hwinner₂ Hstate") as "(>-> & _)". done. }
-    (* contradiction: front authority is strictly less than front lower bound *)
-    iDestruct (front_valid with "Hfront_auth Hfront_lb") as %?. lia.
+    iIntros "% Hstate".
+    destruct state.
+    - iDestruct "Hstate" as "(:inv_state_empty)". lia.
+    - done.
+    - iDestruct "Hstate" as "(:inv_state_emptyish)". lia.
+    - iDestruct "Hstate" as "(:inv_state_superempty)". lia.
+  Qed.
+  #[local] Lemma inv_state_Superempty γ state front back hist lhist vs prophs :
+    back < front →
+    inv_state γ state Unstable front back hist lhist vs prophs -∗
+    ⌜state = Superempty⌝.
+  Proof.
+    iIntros "% Hstate".
+    destruct state.
+    - iDestruct "Hstate" as "(:inv_state_empty lazy=)". done.
+    - iDestruct "Hstate" as "(:inv_state_nonempty lazy=)". done.
+    - iDestruct "Hstate" as "(:inv_state_emptyish lazy=)". lia.
+    - done.
+  Qed.
+  #[local] Lemma inv_state_winner_pop γ state stable front2 back hist lhist vs prophs front1 P :
+    inv_state γ state stable front1 back hist lhist vs prophs -∗
+    winner_pop γ front2 P -∗
+      ∃ P_,
+      ⌜front1 = front2⌝ ∗
+      ▷ (P ≡ P_) ∗
+      ( inv_state_nonempty_steal γ stable front2 back hist lhist vs prophs P_
+      ∨ inv_state_emptyish_steal γ stable front2 back hist lhist P_
+      ) ∗
+      winner_pop γ front2 P.
+  Proof.
+    iIntros "Hstate Hwinner_pop".
+    destruct state.
+    - iDestruct "Hstate" as "(:inv_state_empty)".
+      iDestruct "Hwinner" as "(:winner =3)".
+      iDestruct (winner_pop_exclusive with "Hwinner_pop Hwinner_pop_3") as %[].
+    - iDestruct "Hstate" as "(:inv_state_nonempty)".
+      iDestruct "Hwinner" as "[(:winner =3) | Hwinner]".
+      + iDestruct (winner_pop_exclusive with "Hwinner_pop Hwinner_pop_3") as %[].
+      + destruct prophs as [| id prophs]; first done.
+        iDestruct "Hwinner" as "(%P_ & Hid & Hwinner_steal & HP)".
+        iDestruct (winner_agree with "Hwinner_pop Hwinner_steal") as "#(<- & $)".
+        iSteps.
+    - iDestruct "Hstate" as "(:inv_state_emptyish)".
+      iDestruct "Hwinner" as "[Hwinner_pop_ | (Hwinner_steal & HP)]".
+      + iDestruct (winner_pop_exclusive with "Hwinner_pop Hwinner_pop_") as %[].
+      + iDestruct (winner_agree with "Hwinner_pop Hwinner_steal") as "#(<- & $)".
+        iSteps.
+    - iDestruct "Hstate" as "(:inv_state_superempty)".
+      iDestruct "Hwinner" as "(:winner =3)".
+      iDestruct (winner_pop_exclusive with "Hwinner_pop Hwinner_pop_3") as %[].
+  Qed.
+  #[local] Lemma inv_state_winner_steal γ state stable front2 back hist lhist vs prophs front1 P :
+    inv_state γ state stable front1 back hist lhist vs prophs -∗
+    winner_steal γ front2 P -∗
+      ∃ P_,
+      ⌜front1 = front2⌝ ∗
+      ▷ (P_ ≡ P) ∗
+      inv_state_emptyish_pop γ stable front2 back hist lhist P_ ∗
+      winner_steal γ front2 P.
+  Proof.
+    iIntros "Hstate Hwinner_steal".
+    destruct state.
+    - iDestruct "Hstate" as "(:inv_state_empty)".
+      iDestruct "Hwinner" as "(:winner =3)".
+      iDestruct (winner_steal_exclusive with "Hwinner_steal Hwinner_steal_3") as %[].
+    - iDestruct "Hstate" as "(:inv_state_nonempty)".
+      destruct prophs as [| id prophs].
+      + iDestruct "Hwinner" as "[(:winner =3) | []]".
+        iDestruct (winner_steal_exclusive with "Hwinner_steal Hwinner_steal_3") as %[].
+      + iDestruct "Hwinner" as "[(:winner =3) | (%P_ & Hid & Hwinner_steal_ & HP)]".
+        * iDestruct (winner_steal_exclusive with "Hwinner_steal Hwinner_steal_3") as %[].
+        * iDestruct (winner_steal_exclusive with "Hwinner_steal Hwinner_steal_") as %[].
+    - iDestruct "Hstate" as "(:inv_state_emptyish)".
+      iDestruct "Hwinner" as "[Hwinner_pop | (Hwinner_steal_ & _)]".
+      + iDestruct (winner_agree with "Hwinner_pop Hwinner_steal") as "#(<- & $)".
+        iSteps.
+      + iDestruct (winner_steal_exclusive with "Hwinner_steal Hwinner_steal_") as %[].
+    - iDestruct "Hstate" as "(:inv_state_superempty)".
+      iDestruct "Hwinner" as "(:winner =3)".
+      iDestruct (winner_steal_exclusive with "Hwinner_steal Hwinner_steal_3") as %[].
   Qed.
 
   Lemma inf_ws_queue_1_create_spec ι :
@@ -884,61 +843,523 @@ Section inf_ws_queue_1_G.
       RET t;
       inf_ws_queue_1_inv t ι ∗
       inf_ws_queue_1_model t [] ∗
-      inf_ws_queue_1_owner t
+      inf_ws_queue_1_owner t []
     }}}.
   Proof.
     iIntros "%Φ _ HΦ".
 
     wp_rec.
 
-    (* → [Proph] *)
-    wp_apply (wise_prophet_wp_proph with "[//]") as "%pid %γ_prophet %prophs Hprophet_model".
+    wp_apply (wise_prophets_wp_proph with "[//]") as "%pid %γ_prophet %prophss Hprophet_model".
+    wp_apply (inf_array_create_spec with "[//]") as "%data (#Hdata_inv & Hdata_model)".
+    iDestruct (inf_array_model_to_model'_constant 1 with "Hdata_model") as "Hdata_model".
+    wp_block l as "Hmeta" "(Hl_front & Hl_back & Hl_data & Hl_proph & _)".
+    iMod (pointsto_persist with "Hl_data") as "#Hl_data".
+    iMod (pointsto_persist with "Hl_proph") as "#Hl_proph".
 
-    (* → [inf_array_create ()] *)
-    wp_apply (inf_array_create_spec with "[//]") as "%data (#Harray_inv & Harray_model)".
-
-    (* → [{ #0; #0; data; #pid }] *)
-    wp_block l as "Hmeta" "(Hfront & Hback & Hdata & Hpid & _)".
-    iMod (pointsto_persist with "Hdata") as "#Hdata".
-    iMod (pointsto_persist with "Hpid") as "#Hpid".
-
-    iApply "HΦ".
-
-    iMod clt_alloc as "(%γ_ctl & Hctl₁ & Hctl₂)".
+    iMod model_owner_alloc as "(%γ_model & %γ_owner & Hmodel₁ & Hmodel₂ & Howner₁ & Howner₂)".
     iMod front_alloc as "(%γ_front & Hfront_auth)".
     iMod history_alloc as "(%γ_history & Hhist_auth)".
-    iMod model_alloc as "(%γ_model & Hmodel₁ & Hmodel₂)".
-    iMod lock_alloc as "(%γ_lock & Hlock)".
-    iMod winner_alloc as "(%γ_winner & Hwinner)".
+    iMod winner_alloc as "(%γ_winner & Hwinner_pop & Hwinner_steal)".
 
     set γ := {|
       metadata_data := data ;
+      metadata_inv := ι ;
       metadata_prophet := pid ;
-      metadata_ctl := γ_ctl ;
-      metadata_front := γ_front ;
-      metadata_hist := γ_history ;
-      metadata_model := γ_model ;
-      metadata_lock := γ_lock ;
       metadata_prophet_name := γ_prophet ;
+      metadata_model := γ_model ;
+      metadata_owner := γ_owner ;
+      metadata_front := γ_front ;
+      metadata_history := γ_history ;
       metadata_winner := γ_winner ;
     |}.
     iMod (meta_set γ with "Hmeta") as "#Hmeta"; first done.
 
-    iSplitR "Hctl₂ Hmodel₂ Hlock".
-    { repeat iExists _. iFrame "#∗". iSplitR; first done.
-      iApply inv_alloc. iExists 0, 0%Z, [], [], (λ _, ()%V), [], prophs. iFrame.
-      do 2 (iSplit; first done).
-      unfold_state. iLeft. iFrame. unfold_state. iFrame. done.
-    }
-    iSplitL "Hmodel₂".
-    { iExists l, γ. naive_solver. }
-    iExists l, γ, 0%Z, (λ _, ()%V). iFrame "#∗". done.
+    iApply "HΦ".
+    iSplitR "Howner₁ Hmodel₁"; last iSteps.
+    iExists l, γ. iStep 6.
+    iApply inv_alloc.
+    iExists Empty, Stable, 1, 1, [()%V], [inhabitant], [], (λ _, ()%V), (λ _, []), prophss. iFrameSteps.
   Qed.
 
-  Lemma inf_ws_queue_1_push_spec t ι v :
+  #[local] Lemma front_spec l γ :
+    {{{
+      inv' l γ
+    }}}
+      (#l).{front}
+    {{{ front,
+      RET #front;
+      front_lb γ front
+    }}}.
+  Proof.
+    iIntros "%Φ #Hinv HΦ".
+
+    iInv "Hinv" as "(:inv_inner)".
+    wp_load.
+    iDestruct (front_lb_get with "Hfront_auth") as "#Hfront_lb_1".
+    iSplitR "HΦ". { iFrameSteps. }
+    iSteps.
+  Qed.
+  #[local] Lemma front_spec_owner_Stable l γ back priv ws :
+    {{{
+      inv' l γ ∗
+      owner₁ γ Stable back priv ws
+    }}}
+      (#l).{front}
+    {{{ front,
+      RET #front;
+      owner₁ γ Stable back priv ws ∗
+      front_lb γ front ∗
+      ⌜front ≤ back⌝
+    }}}.
+  Proof.
+    iIntros "%Φ (#Hinv & Howner₁) HΦ".
+
+    iInv "Hinv" as "(:inv_inner =1)".
+    wp_load.
+    iDestruct (owner_agree with "Howner₁ Howner₂") as %(<- & <- & <-).
+    iDestruct (front_lb_get with "Hfront_auth") as "#Hfront_lb".
+    iDestruct (inv_state_Stable with "Hstate") as "#(_ & %)"; first done.
+    iSplitR "Howner₁ HΦ". { iFrameSteps. }
+    iSteps.
+  Qed.
+  #[local] Lemma front_spec_owner_Unstable l γ back priv ws :
+    {{{
+      inv' l γ ∗
+      owner₁ γ Unstable back priv ws
+    }}}
+      (#l).{front}
+    {{{ front,
+      RET #front;
+      owner₁ γ Unstable back priv ws ∗
+      front_lb γ front ∗
+      ⌜front = back ∨ front = S back⌝
+    }}}.
+  Proof.
+    iIntros "%Φ (#Hinv & Howner₁) HΦ".
+
+    iInv "Hinv" as "(:inv_inner =1)".
+    wp_load.
+    iDestruct (owner_agree with "Howner₁ Howner₂") as %(<- & <- & <-).
+    iDestruct (front_lb_get with "Hfront_auth") as "#Hfront_lb".
+    iDestruct (inv_state_Unstable with "Hstate") as "#(_ & %)".
+    iSplitR "Howner₁ HΦ". { iFrameSteps. }
+    iSteps.
+  Qed.
+  #[local] Lemma front_spec_Superempty l γ back priv ws front :
+    back < front →
+    {{{
+      inv' l γ ∗
+      owner₁ γ Unstable back priv ws ∗
+      front_lb γ front
+    }}}
+      (#l).{front}
+    {{{
+      RET #front;
+      owner₁ γ Unstable back priv ws
+    }}}.
+  Proof.
+    iIntros "% %Φ (#Hinv & Howner₁ & #Hfront_lb) HΦ".
+
+    iInv "Hinv" as "(:inv_inner =1)".
+    wp_load.
+    iDestruct (owner_agree with "Howner₁ Howner₂") as %(<- & <- & <-).
+    iDestruct (front_lb_valid with "Hfront_auth Hfront_lb") as %?.
+    iDestruct (inv_state_Superempty with "Hstate") as %->; first lia.
+    iDestruct "Hstate" as "(:inv_state_superempty =1 lazy=)".
+    iSplitR "Howner₁ HΦ". { iExists Superempty. iFrameSteps. }
+    replace (S back) with front by lia.
+    iSteps.
+  Qed.
+  #[local] Lemma front_spec_winner_steal l γ front P :
+    {{{
+      inv' l γ ∗
+      winner_steal γ front P
+    }}}
+      (#l).{front}
+    {{{
+      RET #front;
+      winner_steal γ front P
+    }}}.
+  Proof.
+    iIntros "%Φ (#Hinv & Hwinner_steal) HΦ".
+
+    iInv "Hinv" as "(:inv_inner =1)".
+    wp_load.
+
+    iAssert ⌜front1 = front⌝%I as %->.
+    { iDestruct (inv_state_winner_steal with "Hstate Hwinner_steal") as "(%P_ & $ & _)". }
+
+    iSplitR "Hwinner_steal HΦ". { iFrameSteps. }
+    iSteps.
+  Qed.
+
+  #[local] Lemma back_spec l γ stable back priv ws :
+    {{{
+      inv' l γ ∗
+      owner₁ γ stable back priv ws
+    }}}
+      (#l).{back}
+    {{{
+      RET #back;
+      owner₁ γ stable back priv ws
+    }}}.
+  Proof.
+    iIntros "%Φ (#Hinv & Howner₁) HΦ".
+
+    iInv "Hinv" as "(:inv_inner =1)".
+    wp_load.
+    iDestruct (owner_agree with "Howner₁ Howner₂") as "(<- & <- & <-)".
+    iSplitR "Howner₁ HΦ". { iFrameSteps. }
+    iSteps.
+  Qed.
+
+  #[local] Lemma set_back_spec_Superempty l γ back priv ws front (back' : Z) :
+    back < front →
+    back' = S back →
+    {{{
+      inv' l γ ∗
+      owner₁ γ Unstable back priv ws ∗
+      front_lb γ front
+    }}}
+      #l <-{back} #back'
+    {{{
+      RET ();
+      owner₁ γ Stable (S back) priv ws
+    }}}.
+  Proof.
+    iIntros (? ->) "%Φ (#Hinv & Howner₁ & #Hfront_lb) HΦ".
+
+    iInv "Hinv" as "(:inv_inner =1)".
+    wp_store.
+    iDestruct (owner_agree with "Howner₁ Howner₂") as %(<- & <- & <-).
+    iMod (owner_update Stable (S back) priv with "Howner₁ Howner₂") as "(Howner₁ & Howner₂)".
+    iDestruct (front_lb_valid with "Hfront_auth Hfront_lb") as %?.
+    iDestruct (inv_state_Superempty with "Hstate") as %->; first lia.
+    iDestruct "Hstate" as "(:inv_state_superempty =1 lazy=)".
+    iSplitR "Howner₁ HΦ". { iExists Empty. iFrameSteps. }
+    iSteps.
+  Qed.
+
+  #[local] Lemma inf_array_get_spec_history l γ (i : nat) (i_ : Z) v :
+    i_ = i →
+    {{{
+      inf_array_inv γ.(metadata_data) ∗
+      inv' l γ ∗
+      history_at γ i v
+    }}}
+      inf_array_get γ.(metadata_data) #i_
+    {{{
+      RET v;
+      True
+    }}}.
+  Proof.
+    iIntros (->) "%Φ (#Hdata_inv & #Hinv & #Hhistory_at) HΦ".
+
+    iApply wp_fupd.
+    awp_apply (inf_array_get_spec' with "Hdata_inv") without "HΦ"; first lia.
+    iInv "Hinv" as "(:inv_inner)".
+    iAaccIntro with "Hdata_model"; first iStepFrameSteps. iIntros "Hdata_model".
+
+    iAssert (◇ ⌜(hist ++ vs) !! i = Some v⌝)%I as "#>%Hlookup".
+    { iDestruct (history_at_lookup with "Hhistory_auth Hhistory_at") as %Hlookup.
+      destruct state.
+      - iDestruct "Hstate" as "(:inv_state_empty >)".
+        iPureIntro.
+        apply lookup_app_l_Some; first done.
+      - iDestruct "Hstate" as "(:inv_state_nonempty >)".
+        iPureIntro.
+        destruct vs as [| w vs]; first naive_solver lia.
+        rewrite (assoc (++) hist [w]).
+        apply lookup_app_l_Some; first done.
+      - iDestruct "Hstate" as "(:inv_state_emptyish >)".
+        iPureIntro.
+        apply lookup_app_l_Some; first done.
+      - iDestruct "Hstate" as "(:inv_state_superempty >)".
+        iPureIntro.
+        apply lookup_app_l_Some; first done.
+    }
+
+    iSplitL. { iFrameSteps. }
+    iIntros "!> H£ HΦ".
+
+    rewrite Nat2Z.id decide_True.
+    { eauto using lookup_lt_Some. }
+    erewrite list_lookup_total_correct => //.
+    iApply (lc_fupd_elim_later with "H£ HΦ [//]").
+  Qed.
+  #[local] Lemma inf_array_get_spec_owner l γ back (back_ : Z) priv ws v :
+    back_ = back →
+    priv 0 = v →
+    {{{
+      inf_array_inv γ.(metadata_data) ∗
+      inv' l γ ∗
+      owner₁ γ Stable back priv ws
+    }}}
+      inf_array_get γ.(metadata_data) #back_
+    {{{
+      RET v;
+      owner₁ γ Stable back priv ws
+    }}}.
+  Proof.
+    iIntros (->) "%Hpriv %Φ (#Hdata_inv & #Hinv & Howner₁) HΦ".
+
+    iApply wp_fupd.
+    awp_apply (inf_array_get_spec' with "Hdata_inv") without "HΦ"; first lia.
+    iInv "Hinv" as "(:inv_inner =1)".
+    iAaccIntro with "Hdata_model"; first iStepFrameSteps. iIntros "Hdata_model".
+    iDestruct (owner_agree with "Howner₁ Howner₂") as %(<- & <- & <-).
+    iDestruct (inv_state_Stable with "Hstate") as "#(_ & _ & >->)"; first done.
+    iSplitR "Howner₁". { iFrameSteps. }
+    iIntros "!> H£ HΦ".
+
+    rewrite Nat2Z.id Nat.sub_diag Hpriv decide_False; first lia.
+    iMod (lc_fupd_elim_later with "H£ HΦ") as "HΦ".
+    iSteps.
+  Qed.
+
+  #[local] Lemma inf_array_set_spec_owner {l γ back priv ws} v :
+    {{{
+      inf_array_inv γ.(metadata_data) ∗
+      inv' l γ ∗
+      owner₁ γ Stable back priv ws
+    }}}
+      inf_array_set γ.(metadata_data) #back v
+    {{{
+      RET ();
+      owner₁ γ Stable back (<[0 := v]> priv) ws
+    }}}.
+  Proof.
+    iIntros "%Φ (#Hdata_inv & #Hinv & Howner₁) HΦ".
+
+    iApply wp_fupd.
+    awp_apply (inf_array_set_spec' with "Hdata_inv") without "HΦ"; first lia.
+    iInv "Hinv" as "(:inv_inner =1)".
+    iDestruct (owner_agree with "Howner₁ Howner₂") as %(<- & <- & <-).
+    iAaccIntro with "Hdata_model"; first iStepFrameSteps. iIntros "Hdata_model".
+    iDestruct (inv_state_Stable with "Hstate") as "#(_ & _ & >->)"; first done.
+    rewrite Nat2Z.id Nat.sub_diag decide_False; first lia.
+    iMod (owner_update Stable back (<[0 := v]> priv) with "Howner₁ Howner₂") as "(Howner₁ & Howner₂)".
+    iSplitR "Howner₁". { iFrameSteps. }
+    iIntros "!> H£ HΦ".
+
+    iMod (lc_fupd_elim_later with "H£ HΦ") as "HΦ".
+    iSteps.
+  Qed.
+
+  #[local] Lemma resolve_spec_loser_1 l γ front1 front2 id :
+    front1 < front2 →
+    {{{
+      inv' l γ ∗
+      front_lb γ front2
+    }}}
+      Resolve (CAS (#l).[front]%V #front1 #(front1 + 1)) #γ.(metadata_prophet) (#front1, #id)%V
+    {{{
+      RET #false;
+      True
+    }}}.
+  Proof.
+    iIntros "%Hloser %Φ (#Hinv & #Hfront_lb) HΦ".
+
+    iInv "Hinv" as "(:inv_inner =3)".
+    iDestruct (front_lb_valid with "Hfront_auth Hfront_lb") as %?.
+    wp_apply (wise_prophets_wp_resolve' with "Hprophet_model"); [done.. |].
+    wp_cas as Hcas; zoo_simpl; last lia.
+    iIntros "!> %prophs %Hprophss3 Hprophet_model".
+    iSplitR "HΦ".
+    { iFrameSteps.
+      - iPureIntro => *.
+        rewrite fn_lookup_alter_ne; first lia.
+        auto.
+      - rewrite fn_lookup_insert_ne //. iSteps.
+    }
+    iSteps.
+  Qed.
+  #[local] Lemma resolve_spec_loser_2 l γ front id prophs0 :
+    head prophs0 ≠ Some id →
+    {{{
+      inv' l γ ∗
+      front_lb γ front ∗
+      wise_prophets_full prophet γ.(metadata_prophet_name) front prophs0
+    }}}
+      Resolve (CAS (#l).[front]%V #front #(front + 1)) #γ.(metadata_prophet) (#front, #id)%V
+    {{{
+      RET #false;
+      front_lb γ (S front)
+    }}}.
+  Proof.
+    iIntros "%Hloser %Φ (#Hinv & #Hfront_lb & #Hprophet_full) HΦ".
+
+    iInv "Hinv" as "(:inv_inner =1)".
+    iDestruct (front_lb_valid with "Hfront_auth Hfront_lb") as %?.
+    wp_apply (wise_prophets_wp_resolve' with "Hprophet_model"); [done.. |].
+    wp_apply (wp_cas_nobranch' with "Hl_front") as (b) "%Hcas Hl_front".
+    iIntros "%prophs %Hprophss1 Hprophet_model".
+    destruct b; zoo_simpl.
+
+    - iDestruct (wise_prophets_full_valid with "Hprophet_model Hprophet_full") as %->.
+      rewrite fn_lookup_alter Hpasts1 // in Hloser.
+
+    - iDestruct (front_lb_get with "Hfront_auth") as "#-#Hfront_lb_1".
+      iDestruct (front_lb_le (S front) with "Hfront_lb_1") as "-##Hfront_lb_1"; first lia.
+      iSplitR "HΦ".
+      { iFrameSteps.
+        - iPureIntro => *.
+          rewrite fn_lookup_alter_ne; first lia.
+          auto.
+        - rewrite fn_lookup_insert_ne //. iSteps.
+      }
+      iSteps.
+  Qed.
+  #[local] Lemma resolve_spec_winner_pop l γ front P id :
+    {{{
+      inv' l γ ∗
+      winner_pop γ front P
+    }}}
+      Resolve (CAS (#l).[front]%V #front #(front + 1)) #γ.(metadata_prophet) (#front, #id)%V
+    {{{
+      RET #true;
+      ▷ P
+    }}}.
+  Proof.
+    iIntros "%Φ (#Hinv & Hwinner_pop) HΦ".
+
+    iInv "Hinv" as "(:inv_inner =1)".
+    wp_apply (wise_prophets_wp_resolve' with "Hprophet_model"); [done.. |].
+    wp_apply (wp_cas_nobranch' with "Hl_front") as (b) "%Hcas Hl_front".
+    iIntros "%prophs %Hprophss1 Hprophet_model".
+    iDestruct (inv_state_winner_pop with "Hstate Hwinner_pop") as "(%P_ & -> & #Heq & Hstate & Hwinner_pop)".
+    rewrite Hprophss1.
+    destruct b; zoo_simpl.
+    iMod (front_update with "Hfront_auth") as "Hfront_auth".
+    iDestruct "Hstate" as "[(:inv_state_nonempty_steal =1) | (:inv_state_emptyish_steal =1)]".
+
+    - destruct vs1 as [| v1 vs1] => /=; first naive_solver lia.
+      iDestruct (history_at_get front with "Hhistory_auth") as "#Hhistory_at"; first done.
+
+      iMod "HP" as "(%vs & Hmodel₁ & _ & HP)".
+      iDestruct (model_agree with "Hmodel₁ Hmodel₂") as %->.
+      iMod (model_steal with "Hmodel₁ Hmodel₂") as "(Hmodel₁ & Hmodel₂) /=".
+      iMod ("HP" with "[$Hmodel₁ $Hhistory_at //]") as "HP".
+
+      iSplitR "HP HΦ".
+      { rewrite (assoc _ _ [_]).
+        destruct (decide (S front = back1)) as [<- |].
+
+        - simpl in Hvs1.
+          iExists Empty. iFrameSteps; iPureIntro.
+          + intros.
+            rewrite fn_lookup_alter_ne; first lia.
+            apply Hpasts1; first lia.
+          + simpl_length/=. lia.
+
+        - destruct vs1 as [| v2 vs1] => /=; first naive_solver lia.
+          simpl in Hvs1.
+          iMod (history_update v2 with "Hhistory_auth") as "Hhistory_auth".
+          iExists Nonempty. iFrameSteps; iPureIntro.
+          + intros.
+            rewrite fn_lookup_alter_ne; first lia.
+            apply Hpasts1; first lia.
+          + simpl_length/=. lia.
+      }
+      iIntros "!> {%}".
+
+      iApply "HΦ". iModIntro.
+      iRewrite "Heq" => //.
+
+    - iSplitR "HP HΦ".
+      { iExists Superempty. iFrameSteps. iPureIntro.
+        intros.
+        rewrite fn_lookup_alter_ne; first lia.
+        apply Hpasts1; first lia.
+      }
+      iIntros "!> {%}".
+
+      iApply "HΦ". iModIntro.
+      iRewrite "Heq" => //.
+  Qed.
+  #[local] Lemma resolve_spec_winner_steal l γ front P id :
+    {{{
+      inv' l γ ∗
+      winner_steal γ front P
+    }}}
+      Resolve (CAS (#l).[front]%V #front #(front + 1)) #γ.(metadata_prophet) (#front, #id)%V
+    {{{
+      RET #true;
+      front_lb γ (S front)
+    }}}.
+  Proof.
+    iIntros "%Φ (#Hinv & Hwinner_steal) HΦ".
+
+    iInv "Hinv" as "(:inv_inner =1)".
+    wp_apply (wise_prophets_wp_resolve' with "Hprophet_model"); [done.. |].
+    wp_apply (wp_cas_nobranch' with "Hl_front") as (b) "%Hcas Hl_front".
+    iIntros "%prophs %Hprophss1 Hprophet_model".
+    iDestruct (inv_state_winner_steal with "Hstate Hwinner_steal") as "(%P_ & -> & _ & (:inv_state_emptyish_pop =1) & Hwinner_steal)".
+    destruct b; zoo_simpl.
+    iMod (front_update with "Hfront_auth") as "Hfront_auth".
+    iDestruct (front_lb_get with "Hfront_auth") as "#Hfront_lb".
+    iSplitR "HΦ".
+    { iExists Superempty. iFrameSteps. iPureIntro.
+      intros.
+      rewrite fn_lookup_alter_ne; first lia.
+      apply Hpasts1; first lia.
+    }
+    iSteps.
+  Qed.
+  #[local] Lemma resolve_spec_Empty l γ back priv ws id :
+    {{{
+      inv' l γ ∗
+      owner₁ γ Stable back priv ws ∗
+      front_lb γ back
+    }}}
+      Resolve (CAS (#l).[front]%V #back #(back + 1)) #γ.(metadata_prophet) (#back, #id)%V
+    {{{
+      RET #true;
+      owner₁ γ Unstable back (priv ∘ S) ws ∗
+      front_lb γ (S back) ∗
+      history_at γ back (priv 0)
+    }}}.
+  Proof.
+    iIntros "%Φ (#Hinv & Howner₁ & #Hfront_lb) HΦ".
+
+    iInv "Hinv" as "(:inv_inner =1)".
+    wp_apply (wise_prophets_wp_resolve' with "Hprophet_model"); [done.. |].
+    wp_apply (wp_cas_nobranch' with "Hl_front") as (b) "%Hcas Hl_front".
+    iIntros "%prophs %Hprophss1 Hprophet_model".
+    iDestruct (owner_agree with "Howner₁ Howner₂") as %(<- & <- & <-).
+    iDestruct (front_lb_valid with "Hfront_auth Hfront_lb") as %?.
+    iDestruct (inv_state_Stable with "Hstate") as "#([-> | ->] & _)"; first done.
+
+    - iDestruct "Hstate" as "(:inv_state_empty =1 lazy=)".
+      destruct b; zoo_simpl.
+
+      iMod (front_update with "Hfront_auth") as "Hfront_auth".
+      iClear "Hfront_lb". iDestruct (front_lb_get with "Hfront_auth") as "#Hfront_lb".
+      iMod (history_update (priv 0) with "Hhistory_auth") as "Hhistory_auth".
+      iDestruct (history_at_get with "Hhistory_auth") as "#Hhistory_at"; first done.
+      iMod (owner_update Unstable (length hist1) (priv ∘ S) with "Howner₁ Howner₂") as "(Howner₁ & Howner₂)".
+      iDestruct (inf_array_model'_shift_l' with "Hdata_model") as "Hdata_model".
+      assert (length vs1 = 0) as ->%nil_length_inv by lia.
+      iEval (rewrite app_nil_r -(app_nil_r (hist1 ++ [priv 0]))) in "Hdata_model".
+
+      iSplitR "Howner₁ HΦ".
+      { iExists Superempty. iFrameSteps; iPureIntro.
+        - intros.
+          rewrite fn_lookup_alter_ne; first lia.
+          apply Hpasts1; first lia.
+        - simpl_length/=. lia.
+      }
+      iSteps.
+
+    - iDestruct "Hstate" as "(:inv_state_nonempty =1 lazy=)".
+      exfalso. lia.
+  Qed.
+
+  Lemma inf_ws_queue_1_push_spec t ι ws v :
     <<<
       inf_ws_queue_1_inv t ι ∗
-      inf_ws_queue_1_owner t
+      inf_ws_queue_1_owner t ws
     | ∀∀ vs,
       inf_ws_queue_1_model t vs
     >>>
@@ -946,118 +1367,48 @@ Section inf_ws_queue_1_G.
     <<<
       inf_ws_queue_1_model t (vs ++ [v])
     | RET ();
-      inf_ws_queue_1_owner t
+      inf_ws_queue_1_owner t (vs ++ [v])
     >>>.
   Proof.
-    iIntros "%Φ ((%l & %γ & -> & #Hmeta & #Hdata & #Hpid & #Harray_inv & #Hinv) & (%_l & %_γ & %back & %priv & %Heq & #_Hmeta & Hctl₂ & Hlock)) HΦ". injection Heq as <-.
-    iDestruct (meta_agree with "Hmeta _Hmeta") as %<-. iClear "_Hmeta".
+    iIntros "%Φ ((:inv) & (:owner)) HΦ". injection Heq as <-.
+    iDestruct (meta_agree with "Hmeta Hmeta_") as %<-. iClear "Hmeta_".
 
-    wp_rec. wp_pures.
-
-    (* → [!#l.[back]] *)
-    wp_bind (_.{back})%E.
-    (* open invariant *)
-    iInv "Hinv" as "(%front & %_back & %hist & %vs & %_priv & %past & %prophs & Hfront & Hback & >Hctl₁ & Hfront_auth & Harray_model & Hmodel₁ & >%Hvs & Hprophet_model & >%Hpast & Hstate)".
-    iDestruct (clt_agree with "Hctl₁ Hctl₂") as %(-> & ->).
-    (* do load back *)
+    wp_rec.
+    wp_smart_apply (back_spec with "[$Hinv $Howner₁]") as "Howner₁".
     wp_load.
-    (* we have lock, hence we are in state 1 or state 2, hence [0 ≤ back] *)
-    iAssert ⌜0 ≤ back⌝%I%Z as %Hback.
-    { iDestruct (lock_state with "Hlock Hstate") as "(_ & [Hstate | Hstate])";
-        iDestruct "Hstate" as "(%Hstate & _)"; iPureIntro; lia.
-    }
-    (* close invariant *)
-    iModIntro. iSplitR "Hctl₂ Hlock HΦ".
-    { repeat iExists _. iFrame. done. }
-    clear- Hback.
-
-    (* → [!#l.[data]] *)
-    wp_load.
-
-    (* → [array.(inf_array_set) data #back v] *)
-    awp_apply (inf_array_set_spec' with "Harray_inv") without "HΦ"; first done.
-    (* open invariant *)
-    iInv "Hinv" as "(%front & %_back & %hist & %vs & %_priv & %past & %prophs & Hfront & Hback & >Hctl₁ & Hfront_auth & >Harray_model & Hmodel₁ & >%Hvs & Hprophet_model & >%Hpast & Hstate)".
-    iDestruct (clt_agree with "Hctl₁ Hctl₂") as %(-> & ->).
-    iAaccIntro with "Harray_model"; iIntros "Harray_model".
-    { iFrame. repeat iExists _. iFrame. done. }
-    (* update private values in control tokens *)
-    set (priv' := <[0 := v]> priv).
-    iMod (clt_update back priv' with "Hctl₁ Hctl₂") as "(Hctl₁ & Hctl₂)".
-    (* we have lock, hence we are in state 1 or state 2 *)
-    iDestruct (lock_state with "Hlock Hstate") as "(Hlock & Hstate)".
-    (* hence [front ≤ back] and [length hist = front] *)
-    iAssert (◇ ⌜front ≤ back ∧ length hist = front⌝%Z)%I as "#>%".
-    { iDestruct "Hstate" as "[Hstate | Hstate]";
-        iDestruct "Hstate" as "(>%Hstate & _ & >%Hhist & _)";
-        iPureIntro; lia.
-    }
-    (* hence [back = length (hist ++ vs)] *)
-    assert (₊back = length (hist ++ vs)) as Heq. { simpl_length. lia. }
-    rewrite Heq decide_False; first lia. rewrite Nat.sub_diag.
-    (* close invariant *)
-    iModIntro. iSplitR "Hctl₂ Hlock".
-    { iExists front, back, hist, vs, priv', past, prophs. iFrame.
-      do 2 (iSplit; first auto).
-      unfold_state. iDestruct "Hstate" as "[Hstate | Hstate]"; [iLeft | iRight; iLeft]; done.
-    }
-    iIntros "_ HΦ".
-    clear.
-
+    wp_apply (inf_array_set_spec_owner with "[$Hdata_inv $Hinv $Howner₁]") as "Howner₁".
     wp_pures.
 
-    (* → [#l <-{back} #(back + 1)] *)
-    (* open invariant *)
-    iInv "Hinv" as "(%front & %_back & %hist & %vs & %_priv & %past & %prophs & Hfront & Hback & >Hctl₁ & Hfront_auth & Harray_model & Hmodel₁ & >%Hvs & Hprophet_model & >%Hpast & Hstate)".
-    iDestruct (clt_agree with "Hctl₁ Hctl₂") as %(-> & ->).
-    (* do increment back *)
+    iInv "Hinv" as "(:inv_inner =1)".
     wp_store.
-    (* update private values in control tokens *)
-    set (priv'' i := priv (S i)).
-    iMod (clt_update (back + 1) priv'' with "Hctl₁ Hctl₂") as "(Hctl₁ & Hctl₂)".
-    (* begin transaction *)
-    iMod "HΦ" as "(%_vs & (%_l & %_γ & %Heq & _Hmeta & Hmodel₂) & _ & HΦ)". injection Heq as <-.
-    iDestruct (meta_agree with "Hmeta _Hmeta") as %<-. iClear "_Hmeta".
+    iDestruct (owner_agree with "Howner₁ Howner₂") as %(<- & <- & <-).
+    set priv1 := priv ∘ S.
+    iMod (owner_update Stable (S back) priv1 with "Howner₁ Howner₂") as "(Howner₁ & Howner₂)".
+    iDestruct (inf_array_model'_shift_l with "Hdata_model") as "Hdata_model"; first by intros [].
+    rewrite -(assoc (++)).
+
+    iMod "HΦ" as "(%vs & (:model) & _ & HΦ)". injection Heq as <-.
+    iDestruct (meta_agree with "Hmeta Hmeta_") as %<-. iClear "Hmeta_".
     iDestruct (model_agree with "Hmodel₁ Hmodel₂") as %<-.
-    (* update model values *)
-    set (vs' := vs ++ [v]).
-    iMod (model_update vs' with "Hmodel₁ Hmodel₂") as "(Hmodel₁ & Hmodel₂)".
-    (* end transaction *)
-    iMod ("HΦ" with "[Hmodel₂]") as "HΦ".
-    { repeat iExists _. iFrame "#∗". done. }
-    (* update data model *)
-    iDestruct (inf_array_model'_shift_l with "Harray_model") as "Harray_model"; first by intros [].
-    rewrite -(assoc (++)) -/vs'.
-    (* we have lock, hence we are in state 1 or state 2 *)
-    iDestruct (lock_state with "Hlock Hstate") as "(Hlock & [Hstate | Hstate])".
+    iMod (model_push v with "Howner₁ Hmodel₁ Hmodel₂") as "(Howner₁ & Hmodel₁ & Hmodel₂)".
+    iMod ("HΦ" with "[Hmodel₁]") as "HΦ"; first iFrameSteps.
 
-    - iDestruct "Hstate" as "(%Hstate & Hhist_auth & %Hhist & Hstate)".
-      destruct (nil_or_length_pos vs) as [-> |]; last lia.
-      (* update history values *)
-      iMod (history_update v with "Hhist_auth") as "Hhist_auth".
-      (* close invariant *)
-      iModIntro. iSplitR "Hctl₂ Hlock HΦ".
-      { iExists front, (back + 1)%Z, hist, vs', priv'', past, prophs. iFrame.
-        do 2 (iSplit; first (simpl; auto with lia)).
-        unfold_state. iRight. iLeft. iFrame. iSplit; first auto with lia.
-        unfold_state. destruct (head $ filter _ _) as [[] |]; auto.
-      }
-      clear.
+    iSplitR "Howner₁ HΦ".
+    { iExists Nonempty.
+      iDestruct (inv_state_Stable with "Hstate") as "#(%Hstate1 & _)"; first done.
+      destruct Hstate1 as [-> | ->].
 
-      iApply "HΦ". repeat iExists _. iFrame "#∗". done.
+      - iDestruct "Hstate" as "(:inv_state_empty =1 lazy=)".
+        assert (length vs = 0) as ->%nil_length_inv by lia.
+        iMod (history_update v with "Hhistory_auth") as "Hhistory_auth".
+        iFrameSteps.
 
-    - iDestruct "Hstate" as "(%Hstate & Hhist_auth & %Hhist & Hstate)".
-      destruct vs as [| w vs]; first naive_solver lia.
-      (* close invariant *)
-      iModIntro. iSplitR "Hctl₂ Hlock HΦ".
-      { iExists front, (back + 1)%Z, hist, vs', priv'', past, prophs. iFrame.
-        iSplit. { simpl_length/=. iSteps. }
-        iSplit; first done.
-        unfold_state. iRight. iLeft. iFrame. auto with lia.
-      }
-      clear.
-
-      iApply "HΦ". repeat iExists _. iFrame "#∗". done.
+      - iDestruct "Hstate" as "(:inv_state_nonempty =1 lazy=)".
+        iFrameSteps; iPureIntro.
+        + simpl_length/=. lia.
+        + rewrite take_app_le //; first lia.
+    }
+    iSteps.
   Qed.
 
   Lemma inf_ws_queue_1_steal_spec t ι :
@@ -1073,1014 +1424,380 @@ Section inf_ws_queue_1_G.
       True
     >>>.
   Proof.
-    iIntros "%Φ (%l & %γ & -> & #Hmeta & #Hdata & #Hpid & #Harray_inv & #Hinv) HΦ".
-    iLöb as "IH".
+    iIntros "%Φ (:inv) HΦ".
+
+    iLöb as "HLöb".
 
     wp_rec.
-
-    (* → [Id] *)
-    wp_smart_apply (wp_id with "[//]") as "%id Hid".
-
+    wp_apply (wp_id with "[//]") as (id) "Hid".
+    wp_smart_apply (front_spec with "Hinv") as (front1) "#Hfront_lb_1".
     wp_pures.
 
-    (* → [!#l.[front]] *)
-    wp_bind (_.{front})%E.
-    (* open invariant *)
-    iInv "Hinv" as "(%front1 & %back1 & %hist & %vs & %priv & %past1 & %prophs1 & Hfront & Hback & Hctl₁ & Hfront_auth & Harray_model & Hmodel₁ & >%Hvs & Hprophet_model & >%Hpast1 & Hstate)".
-    (* do load front *)
-    wp_load.
-    (* emit front fragment at [front1] *)
-    iDestruct (front_lb_get with "Hfront_auth") as "#Hfront_lb".
-    (* close invariant *)
-    iModIntro. iSplitR "Hid HΦ".
-    { repeat iExists _. iFrame. done. }
-    clear.
-
-    wp_pures.
-
-    (* → [!#l.[back]] *)
     wp_bind (_.{back})%E.
-    (* open invariant *)
-    iInv "Hinv" as "(%front2 & %back2 & %hist & %vs & %priv & %past2 & %prophs2 & Hfront & Hback & Hctl₁ & Hfront_auth & Harray_model & Hmodel₁ & >%Hvs & Hprophet_model & >%Hpast2 & Hstate)".
-    (* do load back *)
+    iInv "Hinv" as "(:inv_inner =2)".
     wp_load.
-    (* we have [front1 ≤ front2] *)
-    iDestruct (front_valid with "Hfront_auth Hfront_lb") as %Hfront2.
-    (* branching 1: enforce [front1 < back2] *)
-    destruct (decide (front1 < back2)%Z) as [Hbranch1 | Hbranch1]; last first.
-    { (* we have [vs = []] *)
-      assert (length vs = 0) as ->%nil_length_inv by lia.
-      (* begin transaction *)
-      iMod "HΦ" as "(%_vs & (%_l & %_γ & %Heq & #_Hmeta & Hmodel₂) & _ & HΦ)". injection Heq as <-.
-      iDestruct (meta_agree with "Hmeta _Hmeta") as %<-. iClear "_Hmeta".
-      iDestruct (model_agree with "Hmodel₁ Hmodel₂") as %<-.
-      (* end transation *)
-      iMod ("HΦ" with "[Hmodel₂] [//]") as "HΦ".
-      { repeat iExists _. naive_solver. }
-      (* close invariant *)
-      iModIntro. iSplitR "Hid HΦ".
-      { repeat iExists _. iFrame. done. }
-      clear- Hbranch1.
+    iDestruct (front_lb_valid with "Hfront_auth Hfront_lb_1") as %?.
 
-      wp_pures.
+    destruct (decide (front1 < back2)) as [Hbranch1 | Hbranch1]; last first.
+    { assert (length vs2 = 0) as ->%nil_length_inv by lia.
 
-      (* → [if: #(bool_decide (back2 ≤ front1))] *)
-      rewrite bool_decide_eq_true_2; first lia.
+      iMod "HΦ" as "(%vs & (:model) & _ & HΦ)". injection Heq as <-.
+      iDestruct (meta_agree with "Hmeta Hmeta_") as %<-. iClear "Hmeta_".
+      iDestruct (model_agree with "Hmodel₁ Hmodel₂") as %->.
+      iMod ("HΦ" with "[Hmodel₁] [//]") as "HΦ"; first iFrameSteps.
 
-      wp_pures.
-
-      iApply "HΦ".
+      iSplitR "HΦ". { iFrameSteps. }
+      iSteps.
     }
-    (* branching 2: enforce [front2 = front1] *)
-    rewrite Nat.le_lteq in Hfront2. destruct Hfront2 as [Hbranch2 | <-].
-    { (* emit front fragment at [front2] *)
-      iClear "Hfront_lb". iDestruct (front_lb_get with "Hfront_auth") as "#Hfront_lb".
-      (* close invariant *)
-      iModIntro. iSplitR "Hid HΦ".
-      { repeat iExists _. iFrame. done. }
-      clear- Hbranch1 Hbranch2.
+
+    destruct (decide (front1 = front2)) as [<- |]; last first.
+    { assert (front1 < front2) as Hbranch2 by lia.
+      iDestruct (front_lb_get with "Hfront_auth") as "#Hfront_lb_2".
+      iSplitR "HΦ". { iFrameSteps. }
+      iModIntro. clear- Hbranch1 Hbranch2.
 
       wp_pures.
-
-      (* → [if: #(bool_decide (back2 < front1))] *)
       rewrite bool_decide_eq_false_2; first lia.
-
-      (* → [!#l.[prophet]] *)
       wp_load.
-
-      wp_pures.
-
-      (* → [Resolve (CAS #l.[front] #front1 #(front1 + 1)) #γ.(metadata_prophet) (#front1, #id)] *)
-      wp_bind (Resolve (CAS (#l).[front]%V #front1 #(front1 + 1)) #γ.(metadata_prophet) (#front1, #id)%V).
-      (* open invariant *)
-      iInv "Hinv" as "(%front3 & %back3 & %hist & %vs & %priv & %past3 & %prophs3 & Hfront & Hback & Hctl₁ & Hfront_auth & Harray_model & Hmodel₁ & >%Hvs & >Hprophet_model & >%Hpast3 & Hstate)".
-      (* do resolve *)
-      wp_apply (wise_prophet_wp_resolve prophet (front1, id) with "Hprophet_model"); [done.. |].
-      (* branching 3: CAS must fail as we have seen [front2] such that [front1 < front2] *)
-      wp_cas as _Hbranch3 | ->%val_similar_nat; last first.
-      { iDestruct (front_valid with "Hfront_auth Hfront_lb") as %?.
-        lia.
-      }
-      iAssert ⌜front1 < front3⌝%I as %Hbranch3; last clear _Hbranch3.
-      { iDestruct (front_valid with "Hfront_auth Hfront_lb") as %?.
-        auto with lia.
-      }
-      iModIntro. iIntros "%prophs3' -> Hprophet_model".
-      (* close invariant *)
-      iModIntro. iSplitR "Hid HΦ".
-      { iExists front3, back3, hist, vs, priv, (past3 ++ [_]), prophs3'. iFrame.
-        iSplit; first done.
-        iSplit. { iPureIntro. decompose_Forall; done. }
-        unfold_state. iDestruct "Hstate" as "[Hstate | [(%Hstate & Hhist_auth & %Hhist & Hstate) | (Hlock & [(%Hstate & Hhist_auth & %Hhist & Hstate) | Hstate])]]".
-        - iLeft. done.
-        - iRight. iLeft. iFrame. do 2 (iSplit; first done).
-          unfold_state. rewrite filter_cons_False //. lia.
-        - do 2 iRight. iFrame. iLeft. iFrame. do 2 (iSplit; first done).
-          unfold_state. rewrite filter_cons_False //. lia.
-        - do 2 iRight. iFrame.
-      }
-      clear- Hbranch1 Hbranch2 Hbranch3.
-
-      wp_smart_apply domain_yield_spec.
-
-      (* → [inf_ws_queue_1_steal #l] *)
-      wp_smart_apply ("IH" with "HΦ").
+      wp_smart_apply (resolve_spec_loser_1 with "[$Hinv $Hfront_lb_2]") as "_"; first done.
+      iSteps.
     }
-    (* we are in state 2 *)
-    unfold_state. iDestruct "Hstate" as "[(%Hstate & _) | [(_ & Hhist_auth & %Hhist & Hstate) | (_ & [(%Hstate & _) | (%Hstate & _)])]]"; try lia.
-    (* hence there is at least one model value *)
-    destruct vs as [| v vs]; first naive_solver lia.
-    (* emit history fragment at [front1] *)
-    iDestruct (history_at_get front1 v with "Hhist_auth") as "#Hhist_at".
-    { rewrite lookup_app_r; first lia. rewrite Hhist Nat.sub_diag //. }
-    (* emit prophet lower bound at [prophs2] *)
-    iDestruct (wise_prophet_lb_get with "Hprophet_model") as "#Hprophet_lb".
-    (* branching 3: enforce [filter (λ '(_, _, front', _), front' = front1) prophs2 ≠ []] *)
-    unfold_state. destruct (head $ filter _ prophs2) as [(_front1 & id') |] eqn:Hbranch3; first last.
-    { (* close invariant *)
-      iModIntro. iSplitR "Hid HΦ".
-      { iExists front1, back2, hist, (v :: vs), priv, past2, prophs2. iFrame.
-        do 2 (iSplit; first done).
-        unfold_state. iRight. iLeft. iFrame. do 2 (iSplit; first done).
-        unfold_state. rewrite Hbranch3 //.
-      }
-      clear- Hbranch1 Hbranch3.
+
+    iDestruct (wise_prophets_full_get _ front1 with "Hprophet_model") as "#Hprophet_full".
+    iEval (rewrite Hpasts2 //=) in "Hprophet_full".
+
+    destruct (decide (head $ prophss2 front1 = Some id)) as [(prophs0 & Hbranch3)%head_Some | Hbranch3]; last first.
+    { iSplitR "HΦ". { iFrameSteps. }
+      remember (prophss2 front1) as prophs0.
+      iModIntro. clear- Hbranch1 Hbranch3.
 
       wp_pures.
-
-      (* → [if: #(bool_decide (back2 < front1))] *)
       rewrite bool_decide_eq_false_2; first lia.
-
-      (* → [!#l.[prophet]] *)
       wp_load.
-
-      (* inconsistent prophecy resolution *)
-      wp_smart_apply (wp_resolve_inconsistent_1 with "[$Harray_inv $Hinv $Hprophet_lb]") as "% []"; first done.
+      wp_smart_apply (resolve_spec_loser_2 with "[$Hinv $Hfront_lb_1 $Hprophet_full]") as "_"; first done.
+      iSteps.
     }
-    (* branching 4: enforce [id' = id] *)
-    destruct (decide (id' = id)) as [-> | Hbranch4]; first last.
-    { (* close invariant *)
-      iModIntro. iSplitR "Hid HΦ".
-      { iExists front1, back2, hist, (v :: vs), priv, past2, prophs2. iFrame.
-        do 2 (iSplit; first done).
-        unfold_state. iRight. iLeft. iFrame. do 2 (iSplit; first done).
-        unfold_state. rewrite Hbranch3 //.
-      }
-      clear- Hbranch1 Hbranch3 Hbranch4.
+    rewrite Hbranch3.
 
-      wp_pures.
+    iDestruct (inv_state_Nonempty with "Hstate") as %->; first done.
+    iDestruct "Hstate" as "(:inv_state_nonempty =2)".
+    iDestruct "Hwinner" as "[(:winner) | (%P & Hid_ & _)]"; last first.
+    { iDestruct (identifier_model_exclusive with "Hid Hid_") as %[]. }
 
-      (* → [if: #(bool_decide (back2 < front1))] *)
-      rewrite bool_decide_eq_false_2; first lia.
+    destruct vs2 as [| v vs2]; first naive_solver lia.
+    iDestruct (history_at_get front1 with "Hhistory_auth") as "#Hhistory_at"; first done.
+    iMod (winner_update front1 (Φ (Some v)) with "Hwinner_pop Hwinner_steal") as "(Hwinner_pop & Hwinner_steal)".
 
-      (* → [!#l.[prophet]] *)
-      wp_load.
-
-      (* CAS must fail as we are not the winner *)
-      wp_smart_apply (wp_resolve_loser with "[$Harray_inv $Hinv $Hfront_lb $Hprophet_lb]") as "_"; [done.. |].
-
-      wp_smart_apply domain_yield_spec.
-
-      (* → [inf_ws_queue_1_steal #l] *)
-      wp_smart_apply ("IH" with "HΦ").
+    iSplitR "Hwinner_pop".
+    { iExists Nonempty. iFrameSteps.
+      rewrite Hbranch3. iSteps. iIntros "!> !>".
+      rewrite /au. iAuIntro.
+      iApply (aacc_aupd_commit with "HΦ"); first done. iIntros "%vs (:model)". injection Heq as <-.
+      iDestruct (meta_agree with "Hmeta Hmeta_") as %<-. iClear "Hmeta_".
+      iAaccIntro with "Hmodel₁"; first iSteps. iIntros "%v_ %vs' (-> & Hmodel₁ & Hhistory_at_) !>".
+      iDestruct (history_at_agree with "Hhistory_at Hhistory_at_") as %<-.
+      iSteps.
     }
-    (* we now know we are the next winner *)
-    (* we own the winner tokens *)
-    iDestruct "Hstate" as "[(% & % & % & Hwinner₁ & Hwinner₂) | (Hid' & _)]"; last first.
-    { iDestruct (identifier_model_exclusive with "Hid Hid'") as %[]. }
-    (* update winner tokens *)
-    iMod (winner_update front1 Φ with "Hwinner₁ Hwinner₂") as "(Hwinner₁ & Hwinner₂)".
-    (* close invariant *)
-    iModIntro. iSplitR "Hwinner₂".
-    { iExists front1, back2, hist, (v :: vs), priv, past2, prophs2. iFrame.
-      do 2 (iSplit; first done).
-      unfold_state. iRight. iLeft. iFrame. do 2 (iSplit; first done).
-      unfold_state. rewrite Hbranch3. iRight. iFrame.
-      iModIntro. rewrite /au. iAuIntro.
-      iApply (aacc_aupd_commit with "HΦ"); first done. iIntros "%_vs (%_l & %_γ & %Heq & #_Hmeta & Hmodel₂)". injection Heq as <-.
-      iDestruct (meta_agree with "Hmeta _Hmeta") as %<-. iClear "_Hmeta".
-      iAaccIntro with "Hmodel₂".
-      { iIntros "Hmodel₂ !>". iSplitL "Hmodel₂"; last auto.
-        repeat iExists _. iFrame "#∗". done.
-      }
-      iIntros "%w %vs' (-> & Hmodel₂) !>". iSplitL.
-      - repeat iExists _. iSplit; first done. repeat iExists _. naive_solver.
-      - iIntros "HΦ". iApply ("HΦ" with "[//]").
-    }
-    clear- Hbranch1 Hbranch3.
+    iModIntro. clear- Hbranch1.
 
     wp_pures.
-
-    (* → [if: #(bool_decide (back2 < front1))] *)
     rewrite bool_decide_eq_false_2; first lia.
-
-    (* → [!#l.[prophet]] *)
     wp_load.
-
-    wp_pures.
-
-    (* → [Resolve (CAS #l.[front] #front1 #(front1 + 1)) #γ.(metadata_prophet) (#front1, #id)] *)
-    wp_bind (Resolve (CAS (#l).[front]%V #front1 #(front1 + 1)) #γ.(metadata_prophet) (#front1, #id)%V).
-    (* open invariant *)
-    iInv "Hinv" as "(%front3 & %back3 & %hist & %vs & %priv & %past3 & %prophs3 & Hfront & Hback & Hctl₁ & Hfront_auth & Harray_model & Hmodel₁ & >%Hvs & >Hprophet_model & >%Hpast3 & Hstate)".
-    (* we are in state 2 or state 3.1 *)
-    iDestruct (winner₂_state with "Hwinner₂ Hstate") as "(>-> & Hstate)".
-    (* do resolve *)
-    wp_apply (wise_prophet_wp_resolve prophet (front1, id) with "Hprophet_model"); [done.. |].
-    (* CAS must succeed as we are the next winner *)
-    wp_cas_suc.
-    (* branching 5 *)
-    iDestruct "Hstate" as "[Hstate | Hstate]".
-
-    (* branch 5.1: state 2 *)
-    - iDestruct "Hstate" as "(%Hstate & Hhist_auth & %Hhist & %id' & %Φ' & %Hprophs3 & Hwinner₁ & Hwinner₂ & Hid' & HΦ')".
-      iDestruct (winner_agree ‘Some( v ) with "Hwinner₁ Hwinner₂") as "(_ & HΦ & Hwinner₁ & Hwinner₂)".
-      iModIntro. iIntros "%prophs3' -> Hprophet_model".
-      (* update front *)
-      iMod (front_auth_update (S front1) with "Hfront_auth") as "Hfront_auth"; first lia.
-      (* begin transaction *)
-      iMod "HΦ'" as "(%_vs & Hmodel₂ & _ & HΦ')".
-      iDestruct (model_agree with "Hmodel₁ Hmodel₂") as %<-.
-      (* update model values *)
-      destruct vs as [| _v vs]; first naive_solver lia.
-      iAssert ⌜_v = v⌝%I as %->.
-      { (* exploit history fragment *)
-        iDestruct (history_agree with "Hhist_auth Hhist_at") as %Hlookup.
-        iPureIntro.
-        rewrite lookup_app_r in Hlookup; first lia.
-        rewrite list_lookup_singleton_Some in Hlookup. naive_solver.
-      }
-      iMod (model_update vs with "Hmodel₁ Hmodel₂") as "(Hmodel₁ & Hmodel₂)".
-      (* end transaction *)
-      iMod ("HΦ'" with "[$Hmodel₂ //]") as "HΦ'".
-      (* close invariant *)
-      iSplitR "HΦ HΦ'".
-      { simpl in Hvs.
-        iExists (S front1), back3, (hist ++ [v]), vs, priv, (past3 ++ [_]), prophs3'. iFrame.
-        iSplitL "Hfront". { assert (front1 + 1 = S front1)%Z as -> by lia. done. }
-        iSplitL "Harray_model". { rewrite -(assoc (++)) //. }
-        iSplitR; first auto with lia.
-        iSplitR.
-        { iPureIntro. rewrite Forall_app Forall_singleton. split; last lia.
-          eapply Forall_impl; first done. intros (? & ?) ?. lia.
-        }
-        unfold_state. destruct vs as [| w vs]; simpl in Hvs.
-        - iModIntro. iLeft. iFrame. iSplit; first auto with lia.
-          iSplit. { simpl_length/=. auto with lia. }
-          repeat iExists _. iFrame.
-        - iMod (history_update w with "Hhist_auth") as "Hhist_auth".
-          iModIntro. iRight. iLeft. iFrame. iSplit; first auto with lia.
-          iSplit. { simpl_length/=. auto with lia. }
-          unfold_state. destruct (head $ filter _ prophs3') as [[] |].
-          + iLeft. repeat iExists _. iFrame.
-          + repeat iExists _. iFrame.
-      }
-      iModIntro.
-      clear- Hbranch1 Hbranch3.
-
-      (* → [array.(inf_array_get) !#l.[data] #front1] *)
-      wp_smart_apply (inf_array_get_spec_history with "[$Harray_inv $Hinv $Hdata $Hhist_at]") as "_".
-
-      wp_pures.
-
-      iRewrite -"HΦ". done.
-
-    (* branch 5.2: state 3.1 *)
-    - iDestruct "Hstate" as "(-> & Hlock & Hhist_auth & %Hhist & %id' & %Φ' & %Hprophs3 & Hwinner₁ & Hwinner₂ & HΦ')".
-      iDestruct (winner_agree ‘Some( v ) with "Hwinner₁ Hwinner₂") as "(_ & HΦ & Hwinner₁ & Hwinner₂)".
-      iModIntro. iIntros "%prophs3' -> Hprophet_model".
-      (* we know there is no model value and [hist !!! front1 = v] *)
-      destruct (nil_or_length_pos vs) as [-> |]; last lia.
-      iAssert ⌜hist !!! front1 = v⌝%I as %->.
-      { (* exploit history fragment *)
-        iDestruct (history_agree with "Hhist_auth Hhist_at") as %Hlookup.
-        iPureIntro. apply list_lookup_total_correct. done.
-      }
-      (* update front *)
-      iMod (front_auth_update (S front1) with "Hfront_auth") as "Hfront_auth"; first lia.
-      (* close invariant *)
-      iModIntro. iSplitR "HΦ HΦ'".
-      { iExists (S front1), front1, hist, [], priv, (past3 ++ [_]), prophs3'. iFrame.
-        iSplitL "Hfront". { assert (front1 + 1 = S front1)%Z as -> by lia. done. }
-        iSplit; first auto with lia.
-        iSplitR.
-        { iPureIntro. rewrite Forall_app Forall_singleton. split; last lia.
-          eapply Forall_impl; first done. intros (? & ?) ?. lia.
-        }
-        unfold_state. do 2 iRight. iFrame. iRight. do 2 (iSplit; first auto with lia).
-        repeat iExists _. iFrame.
-      }
-      clear- Hbranch1 Hbranch3.
-
-      (* → [array.(inf_array_get) !#l.[data] #front1] *)
-      wp_smart_apply (inf_array_get_spec_history with "[$Harray_inv $Hinv $Hdata $Hhist_at]") as "_".
-
-      wp_pures.
-
-      iRewrite -"HΦ". done.
+    wp_smart_apply (resolve_spec_winner_pop with "[$Hinv $Hwinner_pop]") as "HΦ".
+    wp_load.
+    wp_apply (inf_array_get_spec_history with "[$Hdata_inv $Hinv $Hhistory_at]") as "_"; first done.
+    iSteps.
   Qed.
 
-  Lemma inf_ws_queue_1_pop_spec t ι :
+  Inductive pop_state :=
+    | PopNonempty v
+    | PopEmptyishWinner v
+    | PopEmptyishLoser
+    | PopSuperempty.
+  #[local] Lemma inf_ws_queue_1_pop_0_spec (state : pop_state) l γ stable back (back_ : Z) priv ws id :
+    back_ = back →
+    {{{
+      l.[data] ↦□ γ.(metadata_data) ∗
+      l.[proph] ↦□ #γ.(metadata_prophet) ∗
+      inf_array_inv γ.(metadata_data) ∗
+      inv' l γ ∗
+      owner₁ γ stable back priv ws ∗
+      match state with
+      | PopNonempty v =>
+          ⌜stable = Stable⌝ ∗
+          ⌜priv 0 = v⌝
+      | PopEmptyishWinner v =>
+          ⌜stable = Unstable⌝ ∗
+          history_at γ back v ∗
+          winner_steal γ back inhabitant
+      | PopEmptyishLoser =>
+          ∃ id_winner prophs,
+          ⌜stable = Unstable⌝ ∗
+          wise_prophets_full prophet γ.(metadata_prophet_name) back (id_winner :: prophs) ∗
+          ⌜head (id_winner :: prophs) ≠ Some id⌝
+      | PopSuperempty =>
+          ∃ front,
+          ⌜stable = Unstable⌝ ∗
+          front_lb γ front ∗
+          ⌜front = S back⌝
+      end
+    }}}
+      inf_ws_queue_1_pop_0 #l #id #back_
+    {{{ o back priv,
+      RET o : val;
+      owner₁ γ Stable back priv ws ∗
+      match state with
+      | PopNonempty v =>
+          ⌜o = Some v⌝
+      | PopEmptyishWinner v =>
+          ⌜o = Some v⌝
+      | PopEmptyishLoser =>
+          ⌜o = None⌝
+      | PopSuperempty =>
+          ⌜o = None⌝
+      end
+    }}}.
+  Proof.
+    iIntros (->) "%Φ (#Hl_data & #Hl_proph & #Hdata_inv & #Hinv & Howner₁ & H) HΦ".
+
+    wp_rec. wp_pures.
+    destruct state.
+
+    - iDestruct "H" as "(-> & %Hpriv)".
+      iSpecialize ("HΦ" $! (Some v)).
+
+      wp_apply (front_spec_owner_Stable with "[$Hinv $Howner₁]") as (front2) "(Howner₁ & #Hfront_lb_1 & %Hfront2)".
+      wp_pures.
+      rewrite bool_decide_eq_false_2; first lia.
+      wp_pures.
+      case_bool_decide as Hbranch.
+
+      + wp_load.
+        wp_apply (inf_array_get_spec_owner with "[$Hdata_inv $Hinv $Howner₁]") as "Howner₁"; [lia | done |].
+        iSteps.
+
+      + replace front2 with back by lia.
+
+        wp_load.
+        wp_smart_apply (resolve_spec_Empty with "[$Hinv $Howner₁ $Hfront_lb_1]") as "(Howner₁ & #Hfront_lb_2 & #Hhistory_at)".
+        wp_smart_apply (set_back_spec_Superempty with "[$Hinv $Howner₁ $Hfront_lb_2]") as "Howner₁"; [lia.. |].
+        wp_load.
+        wp_smart_apply (inf_array_get_spec_history with "[$Hdata_inv $Hinv $Hhistory_at]"); first lia.
+        rewrite Hpriv. iSteps.
+
+    - iDestruct "H" as "(-> & #Hhistory_at & Hwinner_steal)".
+      iSpecialize ("HΦ" $! (Some v)).
+
+      wp_apply (front_spec_winner_steal with "[$Hinv $Hwinner_steal]") as "Hwinner_steal".
+      wp_pures.
+      rewrite bool_decide_eq_false_2; first lia.
+      wp_pures.
+      rewrite bool_decide_eq_false_2; first lia.
+      wp_load.
+      wp_smart_apply (resolve_spec_winner_steal with "[$Hinv $Hwinner_steal]") as "#Hfront_lb".
+      wp_smart_apply (set_back_spec_Superempty with "[$Hinv $Howner₁ $Hfront_lb]") as "Howner₁"; [lia.. |].
+      wp_load.
+      wp_apply (inf_array_get_spec_history with "[$Hdata_inv $Hinv $Hhistory_at]"); first done.
+      iSteps.
+
+    - iDestruct "H" as "(%id_winner & %prophs & -> & #Hprophet_full & %Hloser)".
+      iSpecialize ("HΦ" $! None).
+
+      wp_apply (front_spec_owner_Unstable with "[$Hinv $Howner₁]") as (front2) "(Howner₁ & #Hfront_lb_1 & %Hbranch)".
+      wp_pures.
+      destruct Hbranch as [-> | ->].
+
+      + rewrite bool_decide_eq_false_2; first lia.
+        wp_pures.
+        rewrite bool_decide_eq_false_2; first lia.
+        wp_load.
+        wp_smart_apply (resolve_spec_loser_2 with "[$Hinv $Hfront_lb_1 $Hprophet_full]") as "#Hfront_lb_2"; first done.
+        wp_smart_apply (set_back_spec_Superempty with "[$Hinv $Howner₁ $Hfront_lb_2]"); [lia.. |].
+        iSteps.
+
+      + rewrite bool_decide_eq_true_2; first lia.
+        wp_smart_apply (set_back_spec_Superempty with "[$Hinv $Howner₁ $Hfront_lb_1]"); [lia.. |].
+        iSteps.
+
+    - iDestruct "H" as "(%front & -> & #Hfront_lb & ->)".
+      iSpecialize ("HΦ" $! None).
+
+      wp_apply (front_spec_Superempty with "[$Hinv $Howner₁ $Hfront_lb]") as "Howner₁"; first lia.
+      wp_pures.
+      rewrite bool_decide_eq_true_2; first lia.
+      wp_smart_apply (set_back_spec_Superempty with "[$Hinv $Howner₁ $Hfront_lb]") as "Howner₁"; [lia.. |].
+      iSteps.
+  Qed.
+  Lemma inf_ws_queue_1_pop_spec t ι ws :
     <<<
       inf_ws_queue_1_inv t ι ∗
-      inf_ws_queue_1_owner t
+      inf_ws_queue_1_owner t ws
     | ∀∀ vs,
       inf_ws_queue_1_model t vs
     >>>
       inf_ws_queue_1_pop t @ ↑ι
     <<<
-      ∃∃ o,
+      ∃∃ o ws,
       match o with
       | None =>
           ⌜vs = []⌝ ∗
+          ⌜ws = []⌝ ∗
           inf_ws_queue_1_model t []
       | Some v =>
           ∃ vs',
           ⌜vs = vs' ++ [v]⌝ ∗
+          ⌜ws = vs'⌝ ∗
           inf_ws_queue_1_model t vs'
       end
     | RET o;
-      inf_ws_queue_1_owner t
+      inf_ws_queue_1_owner t ws
     >>>.
   Proof.
-    iIntros "%Φ ((%l & %γ & -> & #Hmeta & #Hdata & #Hpid & #Harray_inv & #Hinv) & (%_l & %_γ & %back & %priv & %Heq & #_Hmeta & Hctl₂ & Hlock)) HΦ". injection Heq as <-.
-    iDestruct (meta_agree with "Hmeta _Hmeta") as %<-. iClear "_Hmeta".
+    iIntros "%Φ ((:inv) & (:owner)) HΦ". injection Heq as <-.
+    iDestruct (meta_agree with "Hmeta Hmeta_") as %<-. iClear "Hmeta_".
 
     wp_rec.
-
-    (* → [Id] *)
-    wp_apply (wp_id with "[//]") as "%id Hid".
-
+    wp_apply (wp_id with "[//]") as (id) "Hid".
+    wp_smart_apply (back_spec with "[$Hinv $Howner₁]") as "Howner₁".
     wp_pures.
 
-    (* → [!#l.[back]] *)
-    wp_bind (_.{back})%E.
-    (* open invariant *)
-    iInv "Hinv" as "(%front1 & %_back & %hist & %vs & %_priv & %past1 & %prophs1 & Hfront & Hback & >Hctl₁ & Hfront_auth & Harray_model & Hmodel₁ & >%Hvs & Hprophet_model & >%Hpast1 & Hstate)".
-    iDestruct (clt_agree with "Hctl₁ Hctl₂") as %(-> & ->).
-    (* do load back *)
-    wp_load.
-    (* close invariant *)
-    iModIntro. iSplitR "Hctl₂ Hlock Hid HΦ".
-    { repeat iExists _. iFrame. done. }
-    clear.
-
-    wp_pures.
-
-    (* → [#l.[back] <- #(back - 1)] *)
     wp_bind (_ <-{back} _)%E.
-    (* open invariant *)
-    iInv "Hinv" as "(%front2 & %_back & %hist & %vs & %_priv & %past2 & %prophs2 & Hfront & Hback & >Hctl₁ & Hfront_auth & Harray_model & Hmodel₁ & >%Hvs & Hprophet_model & >%Hpast2 & Hstate)".
-    iDestruct (clt_agree with "Hctl₁ Hctl₂") as %(-> & ->).
-    (* do decrement back *)
+    iInv "Hinv" as "(:inv_inner =1)".
     wp_store.
-    (* update back in control tokens *)
-    iMod (clt_update (back - 1) priv with "Hctl₁ Hctl₂") as "(Hctl₁ & Hctl₂)".
-    (* branching 1 *)
-    (* we have lock, hence we are in state 1 or in state 2 *)
-    (* if we are in state 2, there is either one model value or strictly more than one model value *)
-    iDestruct (lock_state with "Hlock Hstate") as "(Hlock & [Hstate | Hstate])";
-      iDestruct "Hstate" as "(%Hstate & Hhist_auth & %Hhist & Hstate)";
-      last (destruct (Z.lt_total (S front2) back) as [Hstate' | [Hstate' |]]; last lia).
+    iDestruct (owner_agree with "Howner₁ Howner₂") as %(<- & <- & <-).
+    iDestruct (inv_state_Stable with "Hstate") as "#([-> | ->] & _)"; first done.
 
-    (* branch 1.1: [front2 = back]; empty deque *)
-    - subst back.
-      (* emit front fragment at [front2] *)
+    { iDestruct "Hstate" as "(:inv_state_empty =1 lazy=)".
+      assert (0 < back) as Hback by lia.
+      assert (length vs1 = 0) as ->%nil_length_inv by lia.
+
       iDestruct (front_lb_get with "Hfront_auth") as "#Hfront_lb".
-      (* hence there is no model value *)
-      destruct (nil_or_length_pos vs) as [-> |]; last lia.
-      (* begin transaction *)
-      iMod "HΦ" as "(%_vs & (%_l & %_γ & %Heq & #_Hmeta & Hmodel₂) & _ & HΦ)". injection Heq as <-.
-      iDestruct (meta_agree with "Hmeta _Hmeta") as %<-. iClear "_Hmeta".
-      iDestruct (model_agree with "Hmodel₁ Hmodel₂") as %<-.
-      (* end transaction *)
-      iMod ("HΦ" $! None with "[Hmodel₂]") as "HΦ".
-      { iSplit; first done. repeat iExists _. naive_solver. }
-      (* close invariant *)
-      iModIntro. iSplitR "Hctl₂ HΦ".
-      { iExists front2, (front2 - 1)%Z, hist, [], priv, past2, prophs2. iFrame.
-        do 2 (iSplit; first auto with lia).
-        unfold_state. do 2 iRight. iFrame. iRight. iSplit; first auto with lia. naive_solver.
-      }
-      clear.
+      iMod (owner_update Unstable (back - 1) priv with "Howner₁ Howner₂") as "(Howner₁ & Howner₂)".
 
-      wp_pures.
+      iMod "HΦ" as "(%vs & (:model) & _ & HΦ)". injection Heq as <-.
+      iDestruct (meta_agree with "Hmeta Hmeta_") as %<-. iClear "Hmeta_".
+      iDestruct (model_agree with "Hmodel₁ Hmodel₂") as %->.
+      iMod (model_empty with "Howner₁ Hmodel₁ Hmodel₂") as "(Howner₁ & Hmodel₁ & Hmodel₂)".
+      iMod ("HΦ" $! None with "[Hmodel₁]") as "HΦ"; first iFrameSteps.
 
-      (* → [!#l.[front]] *)
-      wp_bind (_.{front})%E.
-      (* open invariant *)
-      iInv "Hinv" as "(%front3 & %_back & %hist & %vs & %_priv & %past3 & %prophs3 & Hfront & Hback & >Hctl₁ & Hfront_auth & Harray_model & Hmodel₁ & >%Hvs & Hprophet_model & >%Hpast3 & Hstate)".
-      iDestruct (clt_agree with "Hctl₁ Hctl₂") as %(-> & ->).
-      (* do load front *)
-      wp_load.
-      (* we are in state 3.2 *)
-      iDestruct (front_state₃₂ with "Hfront_auth Hfront_lb Hstate") as "(-> & Hfront_auth & Hlock & Hstate)"; first done.
-      (* close invariant *)
-      iModIntro. iSplitR "Hctl₂ HΦ".
-      { iExists front2, (front2 - 1)%Z, hist, vs, priv, past3, prophs3. iFrame.
-        do 2 (iSplit; first auto with lia).
-        unfold_state. do 2 iRight. iFrame.
-      }
-      clear.
+      iSplitR "Howner₁ HΦ". { iExists Superempty. iFrameSteps. }
+      iModIntro. clear- Hback.
 
-      wp_pures.
+      wp_smart_apply (inf_ws_queue_1_pop_0_spec PopSuperempty with "[- HΦ]").
+      2: iFrameSteps.
+      1: lia.
+      iSteps.
+    }
 
-      (* → [if: #(bool_decide (back - 1 < back))] *)
-      rewrite bool_decide_eq_true_2; first lia.
+    iDestruct "Hstate" as "(:inv_state_nonempty =1 lazy=)".
+    assert (0 < back) as Hback by lia.
+    destruct vs1 as [| v vs1 _] using rev_ind; first naive_solver lia.
 
-      wp_pures.
+    destruct (decide (S front1 = back)) as [<- | Hbranch1].
 
-      (* → [#l.[back] <- #front2] *)
-      wp_bind (_ <-{back} _)%E.
-      (* open invariant *)
-      iInv "Hinv" as "(%front4 & %_back & %hist & %vs & %_priv & %past4 & %prophs4 & Hfront & Hback & >Hctl₁ & Hfront_auth & Harray_model & Hmodel₁ & >%Hvs & Hprophet_model & >%Hpast4 & Hstate)".
-      iDestruct (clt_agree with "Hctl₁ Hctl₂") as %(-> & ->).
-      (* do increment back *)
-      wp_store.
-      (* update back in control tokens *)
-      iMod (clt_update front2 priv with "Hctl₁ Hctl₂") as "(Hctl₁ & Hctl₂)".
-      (* we are in state 3.2 *)
-      iDestruct (front_state₃₂ with "Hfront_auth Hfront_lb Hstate") as "(-> & Hfront_auth & Hlock & (%state & Hhist_auth & %Hhist & Hstate))"; first done.
-      (* close invariant *)
-      iModIntro. iSplitR "Hctl₂ Hlock HΦ".
-      { iExists front2, front2, hist, vs, priv, past4, prophs4. iFrame.
-        do 2 (iSplit; first auto with lia).
-        unfold_state. iLeft. iFrame. unfold_state. iFrame. done.
-      }
-      clear.
+    - assert (length vs1 = 0) as ->%nil_length_inv.
+      { simpl_length/= in Hvs1. lia. }
+      simpl in *.
 
-      wp_pures.
+      iDestruct (history_at_get front1 with "Hhistory_auth") as "#Hhistory_at"; first done.
+      iMod (owner_update Unstable front1 priv with "Howner₁ Howner₂") as "(Howner₁ & Howner₂)".
+      iEval (rewrite -(app_nil_r (hist1 ++ [v]))) in "Hdata_model".
 
-      iApply "HΦ". repeat iExists _. iFrame "#∗". done.
+      destruct (decide (head $ prophss1 front1 = Some id)) as [(prophs0 & Hprophss1)%head_Some | Hbranch2].
 
-    (* branch 1.2: front2 + 1 < back; no conflict *)
-    - (* there is stricly more than one model value *)
-      destruct vs as [| v vs _] using rev_ind; first naive_solver lia.
-      destruct vs as [| w vs]; rewrite length_app /= in Hvs; first lia.
-      (* update data model *)
-      iEval (rewrite assoc) in "Harray_model".
-      iDestruct (inf_array_model'_shift_r with "Harray_model") as "Harray_model".
-      (* update private values in control tokens *)
-      set (priv' := λ i, match i with 0 => v | S i => priv i end).
-      iMod (clt_update (back - 1) priv' with "Hctl₁ Hctl₂") as "(Hctl₁ & Hctl₂)".
-      (* begin transaction *)
-      iMod "HΦ" as "(%_vs & (%_l & %_γ & %Heq & #_Hmeta & Hmodel₂) & (_ & HΦ))". injection Heq as <-.
-      iDestruct (meta_agree with "Hmeta _Hmeta") as %<-. iClear "_Hmeta".
-      iDestruct (model_agree with "Hmodel₁ Hmodel₂") as %<-.
-      (* update model values *)
-      iMod (model_update (w :: vs) with "Hmodel₁ Hmodel₂") as "(Hmodel₁ & Hmodel₂)".
-      (* end transaction *)
-      iMod ("HΦ" $! (Some v) with "[Hmodel₂]") as "HΦ".
-      { repeat iExists _. iSplit; first done. repeat iExists _. naive_solver. }
-      (* close invariant *)
-      iModIntro. iSplitR "Hctl₂ Hlock HΦ".
-      { iExists front2, (back - 1)%Z, hist, (w :: vs), priv', past2, prophs2. iFrame.
-        do 2 (iSplit; first (simpl; auto with lia)).
-        unfold_state. iRight. iLeft. iFrame. iSplit; auto with lia.
-      }
-      clear.
+      + rewrite Hprophss1.
+        iDestruct "Hwinner" as "[(:winner) | (%id_ & Hid_ & _)]"; last first.
+        { iDestruct (identifier_model_exclusive with "Hid Hid_") as %[]. }
+        iMod (winner_update front1 inhabitant with "Hwinner_pop Hwinner_steal") as "(Hwinner_pop & Hwinner_steal)".
 
-      wp_pures.
+        iMod "HΦ" as "(%vs & (:model) & _ & HΦ)". injection Heq as <-.
+        iDestruct (meta_agree with "Hmeta Hmeta_") as %<-. iClear "Hmeta_".
+        iDestruct (model_agree with "Hmodel₁ Hmodel₂") as %->.
+        iMod (model_pop with "Howner₁ Hmodel₁ Hmodel₂") as "(Howner₁ & Hmodel₁ & Hmodel₂) /=".
+        iMod ("HΦ" $! (Some v) with "[Hmodel₁]") as "HΦ"; first iFrameSteps.
 
-      (* → [!#l.[front]] *)
-      wp_bind (_.{front})%E.
-      (* open invariant *)
-      iInv "Hinv" as "(%front3 & %_back & %hist & %vs & %_priv & %past3 & %prophs3 & Hfront & Hback & >Hctl₁ & Hfront_auth & Harray_model & Hmodel₁ & >%Hvs & Hprophet_model & >%Hpast3 & Hstate)".
-      iDestruct (clt_agree with "Hctl₁ Hctl₂") as %(-> & ->).
-      (* do load front *)
-      wp_load.
-      (* we have lock, hence we are in state 1 or in state 2, hence [front3 ≤ back - 1] *)
-      iAssert ⌜front3 ≤ back - 1⌝%I%Z as %Hfront3.
-      { iDestruct (lock_state with "Hlock Hstate") as "(Hlock & [Hstate | Hstate])";
-          iDestruct "Hstate" as "(%Hstate & _)"; auto with lia.
-      }
-      (* emit front fragment at [front3] *)
-      iDestruct (front_lb_get with "Hfront_auth") as "#Hfront_lb".
-      (* close invariant *)
-      iModIntro. iSplitR "Hctl₂ Hlock HΦ".
-      { repeat iExists _. iFrame. done. }
-      clear- Hfront3.
-
-      wp_pures.
-
-      (* → [if: #(bool_decide (back - 1 < front3))] *)
-      rewrite bool_decide_eq_false_2; first lia.
-
-      wp_pures.
-
-      (* branching 2 *)
-      (* we may or may not have seen an empty deque *)
-      rewrite Z.le_lteq in Hfront3. destruct Hfront3 as [Hfront3 | <-].
-
-      (* branch 2.1: [front3 < back - 1] *)
-      + (* → [if: #(bool_decide (back - 1 < front3))] *)
-        rewrite bool_decide_eq_true_2; first lia.
-
-        (* → [array.(inf_array_get) !#l.[data] #(back - 1)] *)
-        wp_smart_apply (inf_array_get_spec_private with "[$Harray_inv $Hinv $Hdata $Hctl₂ $Hlock]") as "(Hctl₂ & Hlock)"; first done.
-
-        wp_pures.
-
-        rewrite Z.sub_diag /=.
-        iApply "HΦ". repeat iExists _. iFrame "#∗". done.
-
-      (* branch 2.2: [front3 = back - 1] *)
-      + (* → [if: #(bool_decide (front3 < front3))] *)
-        rewrite bool_decide_eq_false_2; first lia.
-
-        (* → [!#l.[prophet]] *)
-        wp_load.
-
-        wp_pures.
-
-        (* → [Resolve (CAS #l.[front] #front3 #(front3 + 1)) #γ.(metadata_prophet) (#front3, #id)] *)
-        wp_bind (Resolve (CAS (#l).[front]%V #front3 #(front3 + 1)) #γ.(metadata_prophet) (#front3, #id)%V).
-        (* open invariant *)
-        iInv "Hinv" as "(%front4 & %_back & %hist & %vs & %_priv & %past4 & %prophs4 & Hfront & Hback & >Hctl₁ & >Hfront_auth & Harray_model & Hmodel₁ & >%Hvs & >Hprophet_model & >%Hpast4 & Hstate)".
-        iDestruct (clt_agree with "Hctl₁ Hctl₂") as %(-> & ->).
-        (* we have lock, hence we are in state 1 or in state 2 *)
-        iDestruct (lock_state with "Hlock Hstate") as "(Hlock & [Hstate | Hstate])";
-          iDestruct "Hstate" as "(>%Hstate & Hhist_auth & >%Hhist & Hstate)";
-          last first.
-        { (* state 2 is actually impossible *)
-          iDestruct (front_valid with "Hfront_auth Hfront_lb") as %?.
-          lia.
+        iSplitR "Howner₁ Hwinner_steal HΦ".
+        { iExists Emptyish. iFrameSteps. iPureIntro.
+          simpl_length/=. lia.
         }
-        apply (inj _) in Hstate as ->.
-        (* do resolve *)
-        wp_apply (wise_prophet_wp_resolve prophet (front3, id) with "Hprophet_model"); [done.. |].
-        (* CAS must succeed *)
-        wp_cas_suc.
-        iModIntro. iIntros "%prophs4' -> Hprophet_model".
-        (* update front authority *)
-        iMod (front_auth_update (S front3) with "Hfront_auth") as "Hfront_auth"; first lia.
-        (* emit front fragment at [front3 + 1] *)
-        iClear "Hfront_lb".
-        iDestruct (front_lb_get with "Hfront_auth") as "#Hfront_lb".
-        (* we know there is no model value *)
-        destruct (nil_or_length_pos vs) as [-> |]; last lia.
-        (* update history values *)
-        set (hist' := hist ++ [v]).
-        iMod (history_update v with "Hhist_auth") as "Hhist_auth".
-        (* emit history fragment at [front3] *)
-        iDestruct (history_at_get front3 v with "Hhist_auth") as "#Hhist_at".
-        { rewrite lookup_app_r; first lia. rewrite Hhist Nat.sub_diag //. }
-        (* update private values in control tokens *)
-        iMod (clt_update front3 priv with "Hctl₁ Hctl₂") as "(Hctl₁ & Hctl₂)".
-        (* update data model *)
-        iDestruct (inf_array_model'_shift_l with "Harray_model") as "Harray_model"; first by intros [].
-        (* close invariant *)
-        iModIntro. iSplitR "Hctl₂ HΦ".
-        { iExists (S front3), front3, (hist ++ [v]), [], priv, (past4 ++ [_]), prophs4'. iFrame.
-          iSplitL "Hfront". { assert (front3 + 1 = S front3)%Z as -> by lia. done. }
-          iSplitL "Harray_model"; first rewrite !right_id //.
-          iSplit; first auto with lia.
-          iSplit.
-          { iPureIntro. rewrite Forall_app Forall_singleton. split; last lia.
-            eapply Forall_impl; first done. intros (? & ?) ?. lia.
+        iIntros "!> {%}".
+
+        wp_smart_apply (inf_ws_queue_1_pop_0_spec (PopEmptyishWinner v) with "[- HΦ]").
+        2: iFrameSteps.
+        1: lia.
+        iSteps.
+
+      + iDestruct "Hwinner" as "[(:winner) | Hwinner]".
+
+        { iMod (winner_update front1 inhabitant with "Hwinner_pop Hwinner_steal") as "(Hwinner_pop & Hwinner_steal)".
+
+          iMod "HΦ" as "(%vs & (:model) & _ & HΦ)". injection Heq as <-.
+          iDestruct (meta_agree with "Hmeta Hmeta_") as %<-. iClear "Hmeta_".
+          iDestruct (model_agree with "Hmodel₁ Hmodel₂") as %->.
+          iMod (model_pop with "Howner₁ Hmodel₁ Hmodel₂") as "(Howner₁ & Hmodel₁ & Hmodel₂) /=".
+          iMod ("HΦ" $! (Some v) with "[Hmodel₁]") as "HΦ"; first iFrameSteps.
+
+          iSplitR "Howner₁ Hwinner_steal HΦ".
+          { iExists Emptyish. iFrameSteps. iPureIntro.
+            simpl_length/=. lia.
           }
-          unfold_state. do 2 iRight. iFrame. iRight. iFrame. iSplit; first auto with lia.
-          simpl_length/=. auto with lia.
+          iIntros "!> {%}".
+
+          wp_smart_apply (inf_ws_queue_1_pop_0_spec (PopEmptyishWinner v) with "[- HΦ]").
+          2: iFrameSteps.
+          1: lia.
+          iSteps.
         }
-        clear.
 
-        wp_pures.
+        iDestruct (wise_prophets_full_get _ front1 with "Hprophet_model") as "#Hprophet_full".
+        iEval (rewrite Hpasts1 //=) in "Hprophet_full".
+        destruct (prophss1 front1) as [| id_winner prophs]; first done.
+        iDestruct "Hwinner" as "(%P & _ & Hwinner_steal & HP)".
 
-        (* → [#l.[back] <- #(front3 + 1)] *)
-        wp_bind (_ <-{back} _)%E.
-        (* open invariant *)
-        iInv "Hinv" as "(%front5 & %_back & %hist & %vs & %_priv & %past5 & %prophs5 & Hfront & Hback & >Hctl₁ & Hfront_auth & Harray_model & Hmodel₁ & >%Hvs & Hprophet_model & >%Hpast5 & Hstate)".
-        iDestruct (clt_agree with "Hctl₁ Hctl₂") as %(-> & ->).
-        (* do increment back *)
-        wp_store.
-        (* update [back] in control tokens *)
-        iMod (clt_update (front3 + 1) priv with "Hctl₁ Hctl₂") as "(Hctl₁ & Hctl₂)".
-        (* we are in state 3.2 *)
-        iDestruct (front_state₃₂ with "Hfront_auth Hfront_lb Hstate") as "(-> & Hfront_auth & Hlock & (%Hstate & Hhist_auth & %Hhist & Hstate))"; first lia.
-        (* close invariant *)
-        iModIntro. iSplitR "Hctl₂ Hlock HΦ".
-        { iExists (S front3), (front3 + 1)%Z, hist, vs, priv, past5, prophs5. iFrame.
-          do 2 (iSplit; first auto with lia).
-          unfold_state. iLeft. iFrame. iSplit; first auto with lia. unfold_state. iFrame. done.
+        iMod "HP" as "(%vs & Hmodel₁ & _ & HP)".
+        iDestruct (model_agree with "Hmodel₁ Hmodel₂") as %->.
+        iMod (model_steal with "Hmodel₁ Hmodel₂") as "(Hmodel₁ & Hmodel₂) /=".
+        iMod ("HP" with "[Hmodel₁]") as "HP"; first iFrameSteps.
+
+        iMod "HΦ" as "(%vs & (:model) & _ & HΦ)". injection Heq as <-.
+        iDestruct (meta_agree with "Hmeta Hmeta_") as %<-. iClear "Hmeta_".
+        iDestruct (model_agree with "Hmodel₁ Hmodel₂") as %->.
+        iMod (model_empty with "Howner₁ Hmodel₁ Hmodel₂") as "(Howner₁ & Hmodel₁ & Hmodel₂)".
+        iMod ("HΦ" $! None with "[Hmodel₁]") as "HΦ"; first iFrameSteps.
+
+        iSplitR "Howner₁ HΦ".
+        { iExists Emptyish. iFrame. iStep 7. iExists P. iSteps. iPureIntro.
+          simpl_length/=. lia.
         }
-        clear.
+        iModIntro. clear- Hbranch2.
 
-        (* → [array.(inf_array_get) !#l.[data] #front3] *)
-        wp_smart_apply (inf_array_get_spec_history with "[$Harray_inv $Hinv $Hdata $Hhist_at]") as "_".
+        wp_smart_apply (inf_ws_queue_1_pop_0_spec PopEmptyishLoser with "[- HΦ]").
+        2: iFrameSteps.
+        1: lia.
+        iSteps.
 
-        wp_pures.
+    - iMod (owner_update Stable (back - 1) (v .: priv) with "Howner₁ Howner₂") as "(Howner₁ & Howner₂)".
+      iEval (rewrite assoc) in "Hdata_model".
+      iDestruct (inf_array_model'_shift_r with "Hdata_model") as "Hdata_model".
 
-        iApply "HΦ". repeat iExists _. iFrame "#∗". done.
+      iMod "HΦ" as "(%vs & (:model) & _ & HΦ)". injection Heq as <-.
+      iDestruct (meta_agree with "Hmeta Hmeta_") as %<-. iClear "Hmeta_".
+      iDestruct (model_agree with "Hmodel₁ Hmodel₂") as %->.
+      iMod (model_pop' with "Howner₁ Hmodel₁ Hmodel₂") as "(Howner₁ & Hmodel₁ & Hmodel₂)".
+      iMod ("HΦ" $! (Some v) with "[Hmodel₁]") as "HΦ"; first iFrameSteps.
 
-    (* branch 1.3: [front2 + 1 = back]; potential conflict *)
-    - subst back.
-      assert (S front2 - 1 = front2)%Z as -> by lia.
-      destruct vs as [| v vs]; simpl in Hvs; first lia.
-      destruct vs; simpl in Hvs; last lia.
-      (* emit front fragment at [front2] *)
-      iDestruct (front_lb_get with "Hfront_auth") as "#Hfront_lb".
-      (* emit history fragment at [front2] *)
-      iDestruct (history_at_get front2 v with "Hhist_auth") as "#Hhist_at".
-      { rewrite lookup_app_r; first lia. rewrite Hhist Nat.sub_diag //. }
-      (* emit prophet lower bound at [prophs2] *)
-      iDestruct (wise_prophet_lb_get with "Hprophet_model") as "#Hprophet_lb".
-      (* branching 2: enforce [filter (λ '(_, _, front', _), front' = front2) prophs2 ≠ []] *)
-      unfold_state. destruct (head $ filter _ prophs2) as [(_front2 & id') |] eqn:Hbranch2; first last.
-      { (* begin transaction *)
-        iMod "HΦ" as "(%_vs & (%_l & %_γ & %Heq & _Hmeta & Hmodel₂) & _ & HΦ)". injection Heq as <-.
-        iDestruct (meta_agree with "Hmeta _Hmeta") as %<-. iClear "_Hmeta".
-        iDestruct (model_agree with "Hmodel₁ Hmodel₂") as %<-.
-        (* update model values *)
-        iMod (model_update [] with "Hmodel₁ Hmodel₂") as "(Hmodel₁ & Hmodel₂)".
-        iDestruct "Hstate" as "(% & % & % & Hwinner₁ & Hwinner₂)".
-        (* end transaction *)
-        iMod ("HΦ" $! (Some v) with "[Hmodel₂]") as "_".
-        { iExists []. iSplit; first done. repeat iExists _. naive_solver. }
-        (* update winner tokens *)
-        iMod (winner_update front2 Φ with "Hwinner₁ Hwinner₂") as "(Hwinner₁ & Hwinner₂)".
-        (* close invariant *)
-        iModIntro. iSplitR "Hctl₂ Hwinner₁".
-        { iExists front2, front2, (hist ++ [v]), [], priv, past2, prophs2. iFrame.
-          iSplitL "Harray_model". { list_simplifier. done. }
-          iSplit. { list_simplifier. auto with lia. }
-          iSplit; first done.
-          unfold_state. do 2 iRight. iFrame. iLeft. iSplit; first done.
-          iSplit. { simpl_length/=. auto with lia. }
-          unfold_state. rewrite Hbranch2. naive_solver.
-        }
-        clear- Hbranch2.
-
-        wp_pures.
-
-        (* → [!#l.[front]] *)
-        wp_bind (_.{front})%E.
-        (* open invariant *)
-        iInv "Hinv" as "(%front3 & %_back & %hist & %vs & %_priv & %past3 & %prophs3 & Hfront & Hback & >Hctl₁ & Hfront_auth & Harray_model & Hmodel₁ & >%Hvs & Hprophet_model & >%Hpast3 & Hstate)".
-        iDestruct (clt_agree with "Hctl₁ Hctl₂") as %(-> & ->).
-        (* do load front *)
-        wp_load.
-        (* we are in state 3.1 *)
-        iDestruct (winner₁_state with "Hwinner₁ Hstate") as "(-> & _ & Hlock & Hhist_auth & %Hhist & %Φ' & %Hprophs3 & Hwinner₁ & Hwinner₂)".
-        (* close invariant *)
-        iModIntro. iSplitR "Hctl₂ Hwinner₁".
-        { iExists front2, front2, hist, vs, priv, past3, prophs3. iFrame.
-          do 2 (iSplit; first done).
-          unfold_state. do 2 iRight. iFrame. iLeft. do 2 (iSplit; first done).
-          unfold_state. rewrite Hprophs3. naive_solver.
-        }
-        clear- Hbranch2.
-
-        wp_pures.
-
-        (* → [if: #(bool_decide (front2 < front2))] *)
-        rewrite bool_decide_eq_false_2; first lia.
-
-        wp_pures.
-
-        (* → [if: #(bool_decide (front2 < front2))] *)
-        rewrite bool_decide_eq_false_2; first lia.
-
-        (* → [!#l.[prophet]] *)
-        wp_load.
-
-        (* inconsistent prophecy resolution *)
-        wp_smart_apply (wp_resolve_inconsistent_1 with "[$Harray_inv $Hinv $Hprophet_lb]") as "% []"; first done.
+      iSplitR "Howner₁ HΦ".
+      { iExists Nonempty. iFrameSteps; iPureIntro.
+        all: simpl_length/= in Hvs1.
+        - lia.
+        - rewrite take_app_le //; first lia.
       }
-      (* branching 3 *)
-      destruct (decide (id' = id)) as [-> | Hbranch3].
+      iModIntro. clear- Hback.
 
-      (* branch 3.1: [id = id']; we are the next winner *)
-      + (* begin transaction *)
-        iMod "HΦ" as "(%_vs & (%_l & %_γ & %Heq & _Hmeta & Hmodel₂) & _ & HΦ)". injection Heq as <-.
-        iDestruct (meta_agree with "Hmeta _Hmeta") as %<-. iClear "_Hmeta".
-        iDestruct (model_agree with "Hmodel₁ Hmodel₂") as %<-.
-        (* update model values *)
-        iMod (model_update [] with "Hmodel₁ Hmodel₂") as "(Hmodel₁ & Hmodel₂)".
-        (* end transaction *)
-        iMod ("HΦ" $! (Some v) with "[Hmodel₂]") as "HΦ".
-        { iExists []. iSplit; first done. repeat iExists _. naive_solver. }
-        (* we own the winner tokens *)
-        iDestruct "Hstate" as "[(% & % & % & Hwinner₁ & Hwinner₂) | (Hid' & _)]"; last first.
-        { iDestruct (identifier_model_exclusive with "Hid Hid'") as %[]. }
-        (* update winner tokens *)
-        set Ψ := (λ v, inf_ws_queue_1_owner #l -∗ Φ v)%I.
-        iMod (winner_update front2 Ψ with "Hwinner₁ Hwinner₂") as "(Hwinner₁ & Hwinner₂)".
-        (* close invariant *)
-        iModIntro. iSplitR "Hctl₂ Hwinner₂".
-        { iExists front2, front2, (hist ++ [v]), [], priv, past2, prophs2. iFrame.
-          iSplitL "Harray_model". { list_simplifier. done. }
-          do 2 (iSplit; first (simpl; auto with lia)).
-          unfold_state. do 2 iRight. iFrame. iLeft. iSplit; first done.
-          iSplit. { simpl_length/=. auto with lia. }
-          unfold_state. rewrite Hbranch2. iFrame.
-          rewrite lookup_total_app_r; first lia. rewrite Hhist Nat.sub_diag //.
-        }
-        clear- Hbranch2.
-
-        wp_pures.
-
-        (* → [!#l.[front]] *)
-        wp_bind (_.{front})%E.
-        (* open invariant *)
-        iInv "Hinv" as "(%front3 & %_back & %hist & %vs & %_priv & %past3 & %prophs3 & Hfront & Hback & >Hctl₁ & Hfront_auth & Harray_model & Hmodel₁ & >%Hvs & Hprophet_model & >%Hpast3 & Hstate)".
-        iDestruct (clt_agree with "Hctl₁ Hctl₂") as %(-> & ->).
-        (* do load front *)
-        wp_load.
-        (* we are in state 3.1, hence [front3 = front2] *)
-        iAssert ⌜front3 = front2⌝%I as %->.
-        { iDestruct (winner₂_state' with "Hwinner₂ Hstate") as "($ & _)". }
-        (* close invariant *)
-        iModIntro. iSplitR "Hctl₂ Hwinner₂".
-        { repeat iExists front2, front2, hist, vs, priv, past3, prophs3. iFrame. done. }
-        clear- Hbranch2.
-
-        wp_pures.
-
-        (* → [if: #(bool_decide (front2 < front2))] *)
-        rewrite bool_decide_eq_false_2; first lia.
-
-        wp_pures.
-
-        (* → [if: #(bool_decide (front2 < front2))] *)
-        rewrite bool_decide_eq_false_2; first lia.
-
-        (* → [!#l.[prophet]] *)
-        wp_load.
-
-        wp_pures.
-
-        (* → [Resolve (CAS #l.[front] #front2 #(front2 + 1)) #γ.(metadata_prophet) (#front2, #id)] *)
-        wp_bind (Resolve (CAS (#l).[front]%V #front2 #(front2 + 1)) #γ.(metadata_prophet) (#front2, #id)%V).
-        (* open invariant *)
-        iInv "Hinv" as "(%front4 & %_back & %hist & %vs & %_priv & %past4 & %prophs4 & Hfront & Hback & >Hctl₁ & Hfront_auth & Harray_model & Hmodel₁ & >%Hvs & >Hprophet_model & >%Hpast4 & Hstate)".
-        iDestruct (clt_agree with "Hctl₁ Hctl₂") as %(-> & ->).
-        (* we are in state 3.1 *)
-        iDestruct (winner₂_state' with "Hwinner₂ Hstate") as "(>-> & Hlock & >Hhist_auth & >%Hhist & %id' & %Ψ' & >%Hprophs4 & Hwinner₁ & Hwinner₂ & HΨ')".
-        iDestruct (winner_agree ‘Some( v ) with "Hwinner₁ Hwinner₂") as "(_ & HΨ & Hwinner₁ & Hwinner₂)".
-        (* exploit history fragment *)
-        iDestruct (history_agree with "Hhist_auth Hhist_at") as %->%list_lookup_total_correct.
-        (* do resolve *)
-        wp_apply (wise_prophet_wp_resolve prophet (front2, id) with "Hprophet_model"); [done.. |].
-        (* CAS must succeed *)
-        wp_cas_suc.
-        iModIntro. iIntros "%prophs4' -> Hprophet_model".
-        (* update front authority *)
-        iMod (front_auth_update (S front2) with "Hfront_auth") as "Hfront_auth"; first lia.
-        (* emit front fragment at [front2 + 1] *)
-        iClear "Hfront_lb".
-        iDestruct (front_lb_get with "Hfront_auth") as "#Hfront_lb".
-        (* close invariant *)
-        iModIntro. iSplitR "Hctl₂ HΨ HΨ'".
-        { iExists (S front2), front2, hist, vs, priv, (past4 ++ [_]), prophs4'. iFrame.
-          iSplitL "Hfront". { assert (front2 + 1 = S front2)%Z as -> by lia. done. }
-          iSplit; first auto with lia.
-          iSplit.
-          { iPureIntro. rewrite Forall_app Forall_singleton. split; last lia.
-            eapply Forall_impl; first done. intros (? & ?) ?. lia.
-          }
-          unfold_state. do 2 iRight. iFrame. iRight. do 2 (iSplit; first auto with lia). repeat iExists _. iFrame.
-        }
-        clear- Hbranch2.
-
-        wp_pures.
-
-        (* → [#l.[back] <- #(front2 + 1)] *)
-        wp_bind (_ <-{back} _)%E.
-        (* open invariant *)
-        iInv "Hinv" as "(%front5 & %_back & %hist & %vs & %_priv & %past5 & %prophs5 & Hfront & Hback & >Hctl₁ & Hfront_auth & Harray_model & Hmodel₁ & >%Hvs & Hprophet_model & >%Hpast5 & Hstate)".
-        iDestruct (clt_agree with "Hctl₁ Hctl₂") as %(-> & ->).
-        (* do increment back *)
-        wp_store.
-        (* update [back] in control tokens *)
-        iMod (clt_update (front2 + 1) priv with "Hctl₁ Hctl₂") as "(Hctl₁ & Hctl₂)".
-        (* we are in state 3.2 *)
-        iDestruct (front_state₃₂ with "Hfront_auth Hfront_lb Hstate") as "(-> & Hfront_auth & Hlock & (%Hstate & Hhist_auth & %Hhist & Hstate))"; first lia.
-        (* close invariant *)
-        iModIntro. iSplitR "Hctl₂ Hlock HΨ HΨ'".
-        { iExists (S front2), (front2 + 1)%Z, hist, vs, priv, past5, prophs5. iFrame.
-          do 2 (iSplit; first auto with lia).
-          unfold_state. iLeft. iFrame. iSplit; first auto with lia. unfold_state. iFrame. done.
-        }
-        clear- Hbranch2.
-
-        (* → [array.(inf_array_get) !#l.[data] #front2] *)
-        wp_smart_apply (inf_array_get_spec_history with "[$Harray_inv $Hinv $Hdata $Hhist_at]") as "_".
-
-        wp_pures.
-
-        iRewrite "HΨ" in "HΨ'". iApply "HΨ'". repeat iExists _. iFrame "#∗". done.
-
-      (* branch 3.2: [id ≠ id']; we are not the next winner *)
-      + (* branching 4 *)
-        iDestruct "Hstate" as "[Hstate | Hstate]".
-
-        (* branch 4.1: winning thief did not show up; contradiction *)
-        * iDestruct "Hstate" as "(% & % & % & Hwinner₁ & Hwinner₂)".
-          (* begin transaction *)
-          iMod "HΦ" as "(%_vs & (%_l & %_γ & %Heq & _Hmeta & Hmodel₂) & _ & HΦ)". injection Heq as <-.
-          iDestruct (meta_agree with "Hmeta _Hmeta") as %<-. iClear "_Hmeta".
-          iDestruct (model_agree with "Hmodel₁ Hmodel₂") as %<-.
-          (* update model values *)
-          iMod (model_update [] with "Hmodel₁ Hmodel₂") as "(Hmodel₁ & Hmodel₂)".
-          (* end transaction *)
-          iMod ("HΦ" $! (Some v) with "[Hmodel₂]") as "HΦ".
-          { iExists []. iSplit; first done. repeat iExists _. naive_solver. }
-          (* update winner tokens *)
-          set Ψ := (λ v, inf_ws_queue_1_owner #l -∗ Φ v)%I.
-          iMod (winner_update front2 Ψ with "Hwinner₁ Hwinner₂") as "(Hwinner₁ & Hwinner₂)".
-          (* close invariant *)
-          iModIntro. iSplitR "Hctl₂ Hwinner₂".
-          { iExists front2, front2, (hist ++ [v]), [], priv, past2, prophs2. iFrame.
-            iSplitL "Harray_model". { list_simplifier. done. }
-            iSplit. { list_simplifier. auto with lia. }
-            iSplit; first done.
-            unfold_state. do 2 iRight. iFrame. iLeft. iSplit; first done.
-            iSplit. { simpl_length/=. auto with lia. }
-            unfold_state. rewrite Hbranch2. iFrame.
-            rewrite lookup_total_app_r; first lia. rewrite Hhist Nat.sub_diag //.
-          }
-          clear- Hbranch2 Hbranch3.
-
-          wp_pures.
-
-          (* → [!#l.[front]] *)
-          wp_bind (_.{front})%E.
-          (* open invariant *)
-          iInv "Hinv" as "(%front3 & %_back & %hist & %vs & %_priv & %past3 & %prophs3 & Hfront & Hback & >Hctl₁ & Hfront_auth & Harray_model & Hmodel₁ & >%Hvs & Hprophet_model & >%Hpast3 & Hstate)".
-          iDestruct (clt_agree with "Hctl₁ Hctl₂") as %(-> & ->).
-          (* do load front *)
-          wp_load.
-          (* we are in state 3.1, hence [front3 = front2] *)
-          iAssert ⌜front3 = front2⌝%I as %->.
-          { iDestruct (winner₂_state' with "Hwinner₂ Hstate") as "($ & _)". }
-          (* close invariant *)
-          iModIntro. iSplitR "Hctl₂ Hwinner₂".
-          { repeat iExists front2, front2, hist, vs, priv, past3, prophs3. iFrame. done. }
-          clear- Hbranch2 Hbranch3.
-
-          wp_pures.
-
-          (* → [if: #(bool_decide (front2 < front2))] *)
-          rewrite bool_decide_eq_false_2; first lia.
-
-          wp_pures.
-
-          (* → [if: #(bool_decide (front2 < front2))] *)
-          rewrite bool_decide_eq_false_2; first lia.
-
-          (* → [!#l.[prophet]] *)
-          wp_load.
-
-          (* inconsistent prophecy resolution *)
-          wp_smart_apply (wp_resolve_inconsistent_2 with "[$Harray_inv $Hinv $Hctl₂ $Hfront_lb $Hprophet_lb $Hwinner₂]"); [done.. |]. iIntros "[]".
-
-        (* branch 4.2: winning thief did show up *)
-        * iDestruct "Hstate" as "(Hid' & %Φ' & Hwinner₁ & HΦ')".
-          (* begin transaction *)
-          iMod "HΦ'" as "(%_vs & Hmodel₂ & _ & HΦ')".
-          iDestruct (model_agree with "Hmodel₁ Hmodel₂") as %<-.
-          (* update model values *)
-          iMod (model_update [] with "Hmodel₁ Hmodel₂") as "(Hmodel₁ & Hmodel₂)".
-          (* end transaction *)
-          iMod ("HΦ'" $! v with "[$Hmodel₂ //]") as "HΦ'".
-          (* begin transaction *)
-          iMod "HΦ" as "(%_vs & (%_l & %_γ & %Heq & _Hmeta & Hmodel₂) & _ & HΦ)". injection Heq as <-.
-          iDestruct (meta_agree with "Hmeta _Hmeta") as %<-. iClear "_Hmeta".
-          iDestruct (model_agree with "Hmodel₁ Hmodel₂") as %<-.
-          (* end transaction *)
-          iMod ("HΦ" $! None with "[Hmodel₂]") as "HΦ".
-          { iSplit; first done. repeat iExists _. iFrame "#∗". done. }
-          (* close invariant *)
-          iModIntro. iSplitR "Hctl₂ HΦ".
-          { iExists front2, front2, (hist ++ [v]), [], priv, past2, prophs2. iFrame.
-            iSplitL "Harray_model". { list_simplifier. done. }
-            iSplit. { list_simplifier. auto with lia. }
-            iSplit; first done.
-            unfold_state. do 2 iRight. iFrame. iLeft. iSplit; first done.
-            iSplit. { simpl_length/=. auto with lia. }
-            unfold_state. rewrite Hbranch2. iFrame.
-            rewrite lookup_total_app_r; first lia. rewrite Hhist Nat.sub_diag //.
-          }
-          clear- Hbranch2 Hbranch3.
-
-          wp_pures.
-
-          (* → [!#l.[front]] *)
-          wp_bind (_.{front})%E.
-          (* open invariant *)
-          iInv "Hinv" as "(%front3 & %_back & %hist & %vs & %_priv & %past3 & %prophs3 & Hfront & Hback & >Hctl₁ & Hfront_auth & Harray_model & Hmodel₁ & >%Hvs & Hprophet_model & >%Hpast3 & Hstate)".
-          iDestruct (clt_agree with "Hctl₁ Hctl₂") as %(-> & ->).
-          (* do load front *)
-          wp_load.
-          (* we are in state 3 *)
-          unfold_state. iDestruct "Hstate" as "[Hstate | [Hstate | Hstate]]";
-            [iDestruct "Hstate" as "(%Hstate & Hhist_auth & %Hhist & Hstate)".. |].
-          { simplify- front3.
-            (* exploit history fragment *)
-            iDestruct (history_agree with "Hhist_auth Hhist_at") as %?%lookup_lt_Some.
-            lia.
-          } {
-            iDestruct (front_valid with "Hfront_auth Hfront_lb") as %?.
-            lia.
-          }
-          (* branching 5 *)
-          iDestruct "Hstate" as "(Hlock & [Hstate | Hstate])";
-            iDestruct "Hstate" as "(%Hstate & Hhist_auth & %Hhist & Hstate)".
-
-          (* branch 5.1: state 3.1; winning thief has not won yet *)
-          --- apply (inj _) in Hstate as ->.
-              (* close invariant *)
-              iModIntro. iSplitR "Hctl₂ HΦ".
-              { iExists front2, front2, hist, vs, priv, past3, prophs3. iFrame.
-                do 2 (iSplit; first done).
-                unfold_state. do 2 iRight. iFrame. iLeft. auto with iFrame.
-              }
-              clear- Hbranch2 Hbranch3.
-
-              wp_pures.
-
-              (* → [if: #(bool_decide (front2 < front2))] *)
-              rewrite bool_decide_eq_false_2; first lia.
-
-              wp_pures.
-
-              (* → [if: #(bool_decide (front2 < front2))] *)
-              rewrite bool_decide_eq_false_2; first lia.
-
-              (* → [!#l.[prophet]] *)
-              wp_load.
-
-              (* CAS must fail as we are not the winner *)
-              wp_smart_apply (wp_resolve_loser with "[$Harray_inv $Hinv $Hfront_lb $Hprophet_lb]"); [done.. |]. iClear "Hfront_lb". iIntros "Hfront_lb".
-
-              wp_pures.
-
-              (* → [#l.[back] <- #(front2 + 1)] *)
-              wp_bind (_ <-{back} _)%E.
-              (* open invariant *)
-              iInv "Hinv" as "(%front5 & %_back & %hist & %vs & %_priv & %past5 & %prophs5 & Hfront & Hback & >Hctl₁ & Hfront_auth & Harray_model & Hmodel₁ & >%Hvs & Hprophet_model & >%Hpast5 & Hstate)".
-              iDestruct (clt_agree with "Hctl₁ Hctl₂") as %(-> & ->).
-              (* do increment back *)
-              wp_store.
-              (* update back in control tokens *)
-              iMod (clt_update (S front2) priv with "Hctl₁ Hctl₂") as "(Hctl₁ & Hctl₂)".
-              (* we are in state 3.2 *)
-              iDestruct (front_state₃₂ with "Hfront_auth Hfront_lb Hstate") as "(-> & Hfront_auth & Hlock & (%state & Hhist_auth & %Hhist & Hstate))"; first lia.
-              (* close invariant *)
-              iModIntro. iSplitR "Hctl₂ Hlock HΦ".
-              { iExists (S front2), (S front2), hist, vs, priv, past5, prophs5. iFrame.
-                iSplitL "Hback". { assert (front2 + 1 = S front2)%Z as -> by lia. done. }
-                do 2 (iSplit; first auto with lia).
-                unfold_state. iLeft. iFrame. unfold_state. iFrame. done.
-              }
-              clear- Hbranch2 Hbranch3.
-
-              wp_pures.
-
-              iApply "HΦ". repeat iExists _. iFrame "#∗". done.
-
-          (* branch 5.2: state 3.2; winning thief has already won *)
-          --- assert (front3 = S front2) as -> by lia.
-              (* emit front fragment at [front2 + 1] *)
-              iClear "Hfront_lb".
-              iDestruct (front_lb_get with "Hfront_auth") as "#Hfront_lb".
-              (* close invariant *)
-              iModIntro. iSplitR "Hctl₂ HΦ".
-              { iExists (S front2), front2, hist, vs, priv, past3, prophs3. iFrame.
-                do 2 (iSplit; first done).
-                unfold_state. do 2 iRight. iFrame. iRight. auto with iFrame.
-              }
-              clear- Hbranch2 Hbranch3.
-
-              wp_pures.
-
-              (* → [if: #(bool_decide (front2 < front2 + 1))] *)
-              rewrite bool_decide_eq_true_2; first lia.
-
-              wp_pures.
-
-              (* → [#l.[back] <- #(front2 + 1)] *)
-              wp_bind (_ <-{back} _)%E.
-              (* open invariant *)
-              iInv "Hinv" as "(%front4 & %_back & %hist & %vs & %_priv & %past4 & %prophs4 & Hfront & Hback & >Hctl₁ & Hfront_auth & Harray_model & Hmodel₁ & >%Hvs & Hprophet_model & >%Hpast4 & Hstate)".
-              iDestruct (clt_agree with "Hctl₁ Hctl₂") as %(-> & ->).
-              (* do increment back *)
-              wp_store.
-              (* update back in control tokens *)
-              iMod (clt_update (S front2) priv with "Hctl₁ Hctl₂") as "(Hctl₁ & Hctl₂)".
-              (* we are in state 3.2 *)
-              iDestruct (front_state₃₂ with "Hfront_auth Hfront_lb Hstate") as "(-> & Hfront_auth & Hlock & (%state & Hhist_auth & %Hhist & Hstate))"; first lia.
-              (* close invariant *)
-              iModIntro. iSplitR "Hctl₂ Hlock HΦ".
-              { iExists (S front2), (S front2), hist, vs, priv, past4, prophs4. iFrame.
-                do 2 (iSplit; first auto with lia).
-                unfold_state. iLeft. iFrame. unfold_state. iFrame. done.
-              }
-              clear- Hbranch2 Hbranch3.
-
-              wp_pures.
-
-              iApply "HΦ". repeat iExists _. iFrame "#∗". done.
+      wp_smart_apply (inf_ws_queue_1_pop_0_spec (PopNonempty v) with "[- HΦ]").
+      2: iFrameSteps.
+      1: lia.
+      iSteps.
   Qed.
 End inf_ws_queue_1_G.
 
